SEARNarith.sml
@@ -121,9 +121,6 @@ val El_def =
                  |> allE (rastt "dot")
                  |> gen_all |> store_as "El_def";
 
-val El_Fun = El_def |> spec_all |> conjE1 |> gen_all
-                    |> store_as "El_Fun";
-
 
 
 val El_eq_eq = prove_store("El_eq_eq",
@@ -159,25 +156,20 @@ e0
  (!u. (u o El(O) = El(a) & u o SUC = f o u) ==> u = Nrec(a,f))”));
 
 
-
+ 
 val App_El_mem = prove_store("App_El_mem",
 e0
 (rpt strip_tac >> dimp_tac >> strip_tac (* 2 *)
- >-- (irule $iffRL FUN_EXT >> rpt strip_tac (* 3 *)
-     >-- (rw[App_El] >> irule $iffRL App_o_l >>
-         arw[App_El,El_Fun]) 
-     >-- (irule o_Fun >> arw[El_Fun]) >>
-     rw[El_Fun]) >>
+ >-- (irule $ iffLR FUN_EXT >> strip_tac >> 
+     arw[App_App_o,El_def,dot_def]) >>
  qby_tac ‘App(f o El(a),dot) = App(El(b),dot)’ 
  >-- arw[] >>
- pop_assum mp_tac >> rw[App_El] >> strip_tac >>
- qsuff_tac ‘App(f o El(a), dot) = App(f,a)’ 
- >-- (strip_tac >> arw[] >> fs[]) >>
- irule $ iffRL App_o_l >>
- arw[El_def])
+ pop_assum mp_tac >> rw[App_App_o,El_def])
 (form_goal
  “!A B f:A->B.!a b. App(f,a) = b <=>
  f o El(a) = El(b)”));
+
+
 
 val Nrec_O_SUC = prove_store("Nrec_O_SUC",
 e0
@@ -234,114 +226,39 @@ e0
   (Pa(f1,g1) = Pa(f2,g2) <=> f1 = f2 & g1 = g2)”));
 
 
-(*
-
-val Thm1_case1_comm_condition_left = prove_store(
-"Thm1_case1_comm_condition_left",
-e0
-(rw[Pa_eq_eq]
-
-
-rpt strip_tac >> qspecl_then [‘N’] assume_tac Id_Fun >>
- drule Pa_distr >> first_x_assum rev_drule >>
- qspecl_then [‘N’,‘O’] assume_tac El_Fun >>
- first_x_assum drule >> arw[idL] >>
- dimp_tac >> strip_tac (* 2 *)
- >-- (drule Pa_eq_eq >> 
-     qby_tac ‘isFun(f o El(O))’ 
-     >-- (irule o_Fun >> arw[El_Fun]) >>
-     first_x_assum drule >> 
-     first_x_assum drule >> first_x_assum rev_drule >>
-     fs[]) >>
- arw[])
-(form_goal
- “!B f:N->B g:1->B. 
- (Pa(Id(N),f) o El(O) = Pa(El(O),g) <=> f o El(O) = g)”));
-
-
-val Thm1_case1_comm_condition_right = prove_store(
-"Thm1_case1_comm_condition_right",
-e0
-(rpt strip_tac >> 
- qsspecl_then [‘SUC o p1(N,B)’,‘h’,‘Pa(id(N),f)’] assume_tac Pa_distr'>>
- qsspecl_then [‘id(N)’,‘f’,‘SUC’] assume_tac Pa_distr' >>
- rfs[] >> 
- assume_tac SUC_Fun >> 
- qspecl_then [‘N’] assume_tac id_Fun >>
- qspecl_then [‘N’,‘B’] assume_tac p1_Fun >>
- qsspecl_then [‘id(N)’,‘f’] assume_tac Pa_Fun >>
- qsspecl_then [‘p1(N,B)’,‘SUC’] assume_tac o_Fun >>
- fs[] >> rfs[] >> fs[] >> rw[o_assoc,idL,idR] >>
- qsspecl_then [‘id(N)’,‘f’] assume_tac p1_of_Pa >> rfs[] >>
- rw[idR] >>
- qsspecl_then [‘SUC’,‘SUC’,‘h o Pa(id(N),f)’,‘f o SUC’] assume_tac Pa_eq_eq' >> 
- qsspecl_then [‘SUC’,‘f’] assume_tac o_Fun >>
- qsspecl_then [‘Pa(id(N),f)’,‘h’] assume_tac o_Fun >>
- fs[] >> rfs[] >> fs[])
-(form_goal
- “!B f:N~>B. isFun(f) ==> !h:N * B ~>B.isFun(h) ==>
- (Pa(SUC o p1(N,B),h) o Pa(id(N),f) = Pa(id(N),f) o SUC <=>
- h o Pa(id(N),f) = f o SUC)”));
 
 val Thm1_case1_comm_condition = prove_store(
 "Thm1_case1_comm_condition",
 e0
-(rpt strip_tac >>  
- drule Thm1_case1_comm_condition_left >> first_x_assum drule >>
- drule Thm1_case1_comm_condition_right >> first_x_assum drule >>
- arw[] >> dimp_tac >> strip_tac >> arw[])
+(rw[Pa_distr,Pa_eq_eq,IdL,o_assoc,p12_of_Pa,IdL,IdR] >>
+(*stupid*)
+rpt strip_tac >> dimp_tac >> strip_tac >> arw[])
 (form_goal
- “!B f0:N~>B g:1~>B h:N * B ~> B.
-  isFun(f0) & isFun(g) & isFun(h) ==> (f0 o El(O) = g & f0 o SUC = h o Pa(id(N),f0) <=>
- Pa(id(N),f0) o El(O) = Pa(El(O),g) &
- Pa(SUC o p1(N,B),h) o Pa(id(N),f0) = Pa(id(N),f0) o SUC)”));
+ “!B f0:N->B g:1->B h:N * B -> B.
+ (f0 o El(O) = g & f0 o SUC = h o Pa(Id(N),f0) <=>
+ Pa(Id(N),f0) o El(O) = Pa(El(O),g) &
+ Pa(SUC o p1(N,B),h) o Pa(Id(N),f0) = Pa(Id(N),f0) o SUC)”));
 
 
 
-val Dot_ex = prove_store("Dot_ex",
-e0
-(rpt strip_tac >> fs[Fun_expand] >>
- first_x_assum (qspecl_then [‘dot’] strip_assume_tac) >>
- last_x_assum (qspecl_then [‘dot’] strip_assume_tac) >>
- rw[dot_def] >> qexists_tac ‘b’ >> arw[] >> rpt strip_tac >>
- first_x_assum irule >> arw[])
-(form_goal
- “!A f:1~>A.isFun(f) ==> ?a. !d.Holds(f,d,a) &
-   (!a0 d. Holds(f,d,a0) ==> a0 = a)”)); 
 
-val Dot_def = Dot_ex |> spec_all |> ex2fsym "Dot" ["f"] 
-                     |> gen_all |> store_as "Dot_def";
+val Dot_def = qdefine_fsym ("Dot",[‘f:1->A’]) ‘App(f:1->A,dot)’
+                           |> gen_all |> store_as "Dot_def";
 
 
-val Holds_El = prove_store("Holds_El",
-e0
-(rpt strip_tac >>  
- qspecl_then [‘A’,‘a’] strip_assume_tac El_def >>
- drule App_def >> arw[] >> flip_tac >> arw[dot_def])
-(form_goal
- “!A a:mem(A) d. Holds(El(a),d,a)”));
-
- 
 val Dot_of_El = prove_store("Dot_of_El",
 e0
-(rpt strip_tac >> qspecl_then [‘A’,‘a’] assume_tac El_Fun >> 
- drule Dot_def >> first_x_assum (qspecl_then [‘dot’] strip_assume_tac) >>
- flip_tac >> first_x_assum irule >> qexists_tac ‘dot’ >>
- rw[Holds_El])
+(rw[El_def,Dot_def])
 (form_goal
  “!A a:mem(A).Dot(El(a)) = a”));
 
 
 val El_of_Dot = prove_store("El_of_Dot",
 e0
-(rpt strip_tac >> irule $ iffRL FUN_EXT >> rw[dot_def] >> rw[El_def] >>
- arw[] >> drule Dot_def >> 
- first_x_assum (qspecl_then [‘dot’] strip_assume_tac) >>
- strip_tac >> flip_tac >> first_x_assum irule >>
- qexists_tac ‘dot’ >> drule Holds_App >> arw[])
+(rw[El_def,Dot_def,dot_def,GSYM FUN_EXT])
 (form_goal
- “!X f:1~>X. isFun(f) ==> El(Dot(f)) = f”));
-*)
+ “!X f:1->X. El(Dot(f)) = f”));
+
 
  
 val to_P_component = prove_store("to_P_component",
@@ -350,80 +267,51 @@ e0
 (form_goal
  “!A B X f:X->A * B.  Pa(p1(A,B) o f,p2(A,B) o f) = f”));
 
-(*
-val is_Nind = Nind_El |> spec_all |> undisch |>spec_all |> conjE2
-                      |> conjE2 |> conjE2
-                      |> disch_all |> gen_all
-                      |> store_as "is_Nind";
+
+val is_Nrec = Nrec_unique 
 
 
+val App_Pa_distr = prove_store("App_Pa_distr",
+e0
+(rpt strip_tac >> 
+ qsspecl_then [‘ App(Pa(f, g), x)’] (assume_tac o GSYM) Pair_component >> 
+ once_arw[] >> rw[Pair_eq_eq,GSYM App_App_o,p12_of_Pa])
+(form_goal
+“!X A f:X->A B g:X->B x. App(Pa(f:X->A,g:X->B),x) = Pair(App(f,x),App(g,x))”));
 
 
 val Thm1_case_1 = prove_store("Thm1_case_1",
 e0
 (rpt strip_tac >> uex_tac >> 
- abbrev_tac “Nind(Dot(Pa(El(O),g:1~>B)),Pa(SUC o p1(N,B),h:N * B~>B)) = f'” >>
- abbrev_tac “p2(N,B) o f':N~>N * B = f” >>
- qspecl_then [‘N’,‘O’] assume_tac El_Fun >>
- qsspecl_then [‘El(O)’,‘g’] assume_tac Pa_Fun >> rfs[] >>
- drule Dot_def >>
- first_x_assum (qspecl_then [‘dot’] strip_assume_tac) >>
- qspecl_then [‘N’,‘B’] strip_assume_tac p12_Fun >>
- assume_tac SUC_Fun >>
- qsspecl_then [‘p1(N,B)’,‘SUC’] assume_tac o_Fun >> rfs[] >>
- qsspecl_then [‘SUC o p1(N,B)’,‘h’] assume_tac Pa_Fun >> rfs[] >>
- qsspecl_then [‘Pa(SUC o p1(N,B),h)’] assume_tac Nind_El >>
- rfs[] >>
- first_x_assum (qspecl_then [‘Dot(Pa(El(O),g))’] strip_assume_tac) >>
- qby_tac ‘isFun(f')’ 
- >-- (qpick_x_assum ‘Nind(Dot(Pa(El(O), g)), Pa(SUC o p1(N, B), h)) = f'’
-      (assume_tac o GSYM)  >> arw[]) >> 
- qsspecl_then [‘f'’,‘p1(N,B)’] assume_tac o_Fun >> rfs[] >>
- qsspecl_then [‘f'’,‘p2(N,B)’] assume_tac o_Fun >> rfs[] >> 
- qby_tac ‘p1(N,B) o f' = id(N)’ >--
- (irule comm_with_SUC_id >> arw[o_assoc] >>  
-  qsspecl_then [‘Pa(El(O),g)’] assume_tac El_of_Dot >> rfs[] >>
-  rw[GSYM o_assoc] >> 
-  qsspecl_then [‘SUC o p1(N,B)’,‘h’] assume_tac p1_of_Pa >> rfs[] >>
-  irule p1_of_Pa >> arw[]) >>
-  qby_tac ‘f' = Pa(id(N),f)’ >-- 
- (qsspecl_then [‘f'’] assume_tac to_P_component >>
-  first_x_assum drule >> once_arw[] >> pop_assum (K all_tac) >> arw[]) >>
+ qabbrev_tac ‘Nrec(Dot(Pa(El(O),g:1->B)),Pa(SUC o p1(N,B),h:N * B->B)) = f'’ >>
+ qabbrev_tac ‘p2(N,B) o f':N->N * B = f’ >>
  qexists_tac ‘f’ >>
- qby_tac ‘f o El(O) = g & f o SUC = h o Pa(id(N), f)’
- >-- (qpick_x_assum ‘p2(N, B) o f' = f’ (assume_tac o GSYM)>>
+ qsspecl_then [‘Dot(Pa(El(O), g))’,‘Pa(SUC o p1(N, B), h)’] strip_assume_tac
+ Nrec_El >> rfs[] >>
+ qby_tac ‘p1(N,B) o f' = Id(N)’ >--
+ (irule comm_with_SUC_id >> arw[o_assoc,p12_of_Pa,El_of_Dot,Pa_distr]) >>
+ qby_tac ‘f' = Pa(Id(N),f)’ >-- 
+ (irule is_Pa >> arw[]) >>
+ qby_tac ‘f o El(O) = g & f o SUC = h o Pa(Id(N), f)’
+ >-- (qpick_x_assum ‘p2(N, B) o f' = f’ (assume_tac o GSYM) >>
       once_arw[] >> pop_assum (K all_tac) >> rw[o_assoc] >> once_arw[] >>
-      rw[GSYM o_assoc] >> 
-      qsspecl_then [‘Pa(El(O),g)’] assume_tac El_of_Dot >> 
-      first_x_assum drule >> arw[] >> 
-      qsspecl_then [‘El(O)’,‘g’] assume_tac p2_of_Pa >> rfs[] >>
-      qsspecl_then [‘SUC o p1(N,B)’,‘h’] assume_tac p2_of_Pa >> rfs[] >>
-      qsspecl_then [‘id(N)’,‘f’] assume_tac p2_of_Pa >> rfs[] >>
-      qspecl_then [‘N’] assume_tac id_Fun >> fs[]) >>
+      rw[GSYM o_assoc] >> arw[p12_of_Pa,El_of_Dot]) >>
  once_arw[] >> rw[] >>  
  rpt strip_tac >>  
- qsuff_tac ‘Pa(id(N), f'') = Pa(id(N), f)’ 
- >-- (strip_tac >> 
-      qsspecl_then [‘id(N)’,‘id(N)’,‘f''’,‘f’] assume_tac Pa_eq_eq' >>
-      qspecl_then [‘N’] assume_tac id_Fun >>
-      fs[] >> rfs[]) >>
- qsuff_tac ‘Pa(id(N), f'') = f'’ >-- arw[] >>
- qsuff_tac ‘Pa(id(N), f'') = 
-  Nind(Dot(Pa(El(O), g)), Pa(SUC o p1(N, B), h))’ >-- arw[] >>
- irule is_Nind >>  
- qsspecl_then [‘id(N)’,‘f''’] assume_tac Pa_Fun >> 
- qspecl_then [‘N’] assume_tac id_Fun >> rfs[] >> fs[] >> 
- qsspecl_then [‘Pa(El(O),g)’] assume_tac El_of_Dot >> rfs[] >>
- qsspecl_then [‘id(N)’,‘f''’,‘SUC’] assume_tac Pa_distr' >> rfs[] >>
- rw[idL] >> 
- qsspecl_then [‘SUC o p1(N,B)’,‘h’,‘Pa(id(N),f'')’] assume_tac
- Pa_distr' >> rfs[] >> rw[o_assoc] >>
- qsspecl_then [‘id(N)’,‘f''’] assume_tac p1_of_Pa >> rfs[] >>
- rw[idR] >>
- qsspecl_then [‘id(N)’,‘f''’,‘El(O)’] assume_tac Pa_distr' >>
- rfs[] >> rw[idL])
+ qsuff_tac ‘Pa(Id(N), f'') = Pa(Id(N), f)’ 
+ >-- rw[Pa_eq_eq] >>
+ qsuff_tac ‘Pa(Id(N), f'') = f'’ >-- arw[] >>
+ qsuff_tac ‘Pa(Id(N), f'') = 
+  Nrec(Dot(Pa(El(O), g)), Pa(SUC o p1(N, B), h))’ >-- arw[] >>
+ irule Nrec_unique >>  
+ arw[Pa_distr,o_assoc,IdL,Dot_def,p12_of_Pa,IdR] >>
+ rw[App_Pa_distr,Pair_eq_eq,Id_def,El_def] >>
+ qby_tac ‘App(f'' o El(O),dot) = App(g,dot)’
+ >-- arw[] >> pop_assum mp_tac >>
+ rw[App_App_o,El_def])
 (form_goal
- “!B g:1~>B h:N * B ~> B. isFun(g) & isFun(h) ==>  ?!f:N~>B. isFun(f) & f o El(O) = g & f o SUC = h o Pa(id(N),f)”));
+ “!B g:1->B h:N * B -> B. 
+   ?!f:N->B. f o El(O) = g & f o SUC = h o Pa(Id(N),f)”));
 
 
 
@@ -433,33 +321,31 @@ val Tp1_ex = prove_store("Tp1_ex",
 e0
 (rpt strip_tac >> qexists_tac ‘Tp(f o p1(A,1))’ >> rw[])
 (form_goal
-“!A B f:A~>B.?tpf:1~>Exp(A,B).Tp(f o p1(A,1)) = tpf”));
+“!A B f:A->B.?tpf:1->Exp(A,B).Tp(f o p1(A,1)) = tpf”));
 
-val Tp1_def = Tp1_ex |> spec_all |> ex2fsym0 "Tp1" ["f"]
+val Tp1_def = Tp1_ex |> spec_all |> qSKOLEM "Tp1" [‘f’]
                      |> gen_all
                      |> store_as "Tp1_def";
 
 
 val Ev_of_Tp = prove_store("Ev_of_Tp",
 e0
-(rpt strip_tac >> drule Tp_def >> arw[])
+(rw[Tp_def])
 (form_goal
- “!A B X f:A * X ~>B. isFun(f) ==>
+ “!A B X f:A * X ->B. 
   Ev(A,B) o Pa(p1(A,X),Tp(f) o p2(A,X)) = f”));
 
 
 val Tp_eq = prove_store("Tp_eq",
 e0
-(rpt strip_tac >> dimp_tac >> strip_tac (* 2 *)
- >-- (drule $ GSYM Ev_of_Tp >> rev_drule $ GSYM Ev_of_Tp >> once_arw[] >>
-      pop_assum (K all_tac) >> pop_assum (K all_tac) >> arw[]) >> arw[])
+(rpt strip_tac >> dimp_tac >> strip_tac >> arw[] >>
+ qsspecl_then [‘f’] assume_tac Ev_of_Tp >>
+ qsspecl_then [‘g’] assume_tac Ev_of_Tp >>
+ rfs[])
 (form_goal
- “!A B X f:A * X ~>B g:A * X ~>B.isFun(f) ==> isFun(g) ==> (Tp(f) = Tp(g) <=> f = g)”));
+ “!A B X f:A * X ->B g:A * X ->B.(Tp(f) = Tp(g) <=> f = g)”));
 
 
-val is_Tp = Tp_def |> strip_all_and_imp |> conjE2
-                   |> disch_all |> gen_all
-                   |> store_as "is_Tp";
 
 
 
@@ -468,12 +354,10 @@ e0
 (rpt strip_tac >> 
  qsuff_tac ‘f = Tp(Ev(A,B) o Pa(p1(A,X),g o p2(A,X))) & 
   g = Tp(Ev(A,B) o Pa(p1(A,X),g o p2(A,X)))’
- >-- (rpt strip_tac >> once_arw[] >> rw[]) >>
- strip_tac (* 2 *) >>
- irule is_Tp >> arw[] >> irule o_Fun >> rw[Ev_Fun] >>
- irule Pa_Fun >> rw[p12_Fun] >> irule o_Fun >> arw[p12_Fun])
+ >-- (rpt strip_tac >> once_arw[] >> rw[]) >> strip_tac 
+ >> irule is_Tp >> arw[])
 (form_goal
- “!A B X f g. isFun(f) & isFun(g) ==> (Ev(A,B) o Pa(p1(A,X),f o p2(A,X)) = 
+ “!A B X f g. (Ev(A,B) o Pa(p1(A,X),f o p2(A,X)) = 
               Ev(A,B) o Pa(p1(A,X),g o p2(A,X)) ==> f = g)”));
 
 
@@ -483,47 +367,19 @@ e0
  qsuff_tac ‘f = Pa(p1(A,B) o g,p2(A,B) o g) &
             g = Pa(p1(A,B) o g,p2(A,B) o g)’ >--
  (strip_tac >> once_arw[] >> rw[]) >>
- strip_tac (* 2 *) >--
- (irule is_Pa >> arw[] >> strip_tac >> irule o_Fun >> arw[p12_Fun]) >>
- drule to_P_component >> first_x_assum accept_tac)
+ strip_tac >> irule is_Pa >> arw[])
 (form_goal
- “!A B X f:X~>A * B g:X~>A * B. isFun(f) & isFun(g) ==> p1(A,B) o f = p1(A,B) o g &
+ “!A B X f:X->A * B g:X->A * B.  p1(A,B) o f = p1(A,B) o g &
  p2(A,B) o f = p2(A,B) o g ==> f = g”));
-
-val Tp_Fun = Tp_def |> strip_all_and_imp |> conjE1 |> conjE1
-                    |> disch_all |> gen_all
-                    |> store_as "Tp_Fun";
-
-
-val Tp1_Fun = prove_store("Tp1_Fun",
-e0
-(rpt strip_tac >> rw[GSYM Tp1_def] >> irule Tp_Fun >>
- irule o_Fun >> arw[p12_Fun])
-(form_goal
- “!A B f:A~>B. isFun(f) ==> isFun(Tp1(f))”));
 
 
 
 val Pa_o_split = prove_store("Pa_o_split",
 e0
 (rpt strip_tac >> irule to_P_eq >>
- qspecl_then [‘A’,‘B’] strip_assume_tac p12_Fun >>
- qspecl_then [‘A’,‘X’] strip_assume_tac p12_Fun >>
- qsspecl_then [‘p2(A,X)’,‘g’] assume_tac o_Fun >> rfs[] >>
- qsspecl_then [‘p2(A,B)’,‘f’] assume_tac o_Fun >> rfs[] >>
- qsspecl_then [‘f o p2(A,B)’,‘g’] assume_tac o_Fun >> rfs[] >>
- qsspecl_then [‘p1(A,B)’,‘g o f o p2(A,B)’] assume_tac Pa_Fun >> rfs[] >>
- qsspecl_then [‘p1(A,X)’,‘g o p2(A,X)’] assume_tac Pa_Fun >> rfs[] >> 
- qsspecl_then [‘p1(A,B)’,‘f o p2(A,B)’] assume_tac Pa_Fun >> rfs[] >>  
- qsspecl_then [‘Pa(p1(A, B), f o p2(A, B))’,‘Pa(p1(A, X), (g o p2(A, X)))’] assume_tac o_Fun >> rfs[] >>
- fs[GSYM o_assoc] >>
- qsspecl_then [‘p1(A,B)’,‘(g o f) o p2(A,B)’] assume_tac p12_of_Pa >>
- rfs[] >> 
- qsspecl_then [‘p1(A,X)’,‘g o p2(A,X)’] assume_tac p12_of_Pa >> rfs[] >>
- fs[o_assoc] >>
- qsspecl_then [‘p1(A,B)’,‘f o p2(A,B)’] assume_tac p12_of_Pa >> rfs[])
+ rw[p12_of_Pa,Pa_distr,o_assoc])
 (form_goal
- “!B X f:B~>X Y g:X~>Y. isFun(f) & isFun(g) ==> !A.Pa(p1(A,B),g:X~>Y o f o p2(A,B)) = 
+ “!B X f:B->X Y g:X->Y.  !A.Pa(p1(A,B),g:X->Y o f o p2(A,B)) = 
   Pa(p1(A,X), g o p2(A,X)) o Pa(p1(A,B),f o p2(A,B))”));
 
 
@@ -531,18 +387,9 @@ val Thm1_comm_eq_left = prove_store(
 "Thm1_comm_eq_left",
 e0
 (rpt strip_tac >> 
- qsspecl_then [‘O’] assume_tac El_Fun >>
- qspecl_then [‘A’,‘1’] strip_assume_tac p12_Fun >>
- qsspecl_then [‘p2(A,1)’,‘El(O)’] assume_tac o_Fun >> rfs[] >>
- qsspecl_then [‘p1(A,1)’,‘El(O) o p2(A,1)’] assume_tac Pa_Fun >> rfs[]>>
- qsspecl_then [‘g’] assume_tac Tp1_Fun >> rfs[] >>
- qsspecl_then [‘f’] assume_tac Tp_Fun >> rfs[] >>
- qspecl_then [‘A’,‘N’] assume_tac p12_Fun >> rfs[] >>
- qsspecl_then [‘p2(A,N)’,‘Tp(f)’] assume_tac o_Fun >> rfs[] >> 
- qsspecl_then [‘p1(A,1)’,‘g’] assume_tac o_Fun >> rfs[]  >>
  qby_tac ‘Pa(p1(A,1), Tp(f) o El(O) o p2(A,1)) = 
  Pa(p1(A,N),Tp(f) o p2(A,N)) o Pa(p1(A,1),El(O) o p2(A,1))’
- >-- (irule Pa_o_split  >> arw[]) >>
+ >-- rw[Pa_o_split] >>
  dimp_tac >> strip_tac (* 2 *)
  >-- (qsuff_tac ‘f o Pa(p1(A, 1), El(O) o p2(A, 1)) = 
                  Ev(A,B) o Pa(p1(A,1),(Tp(f) o El(O)) o p2(A,1)) &
@@ -555,91 +402,48 @@ e0
      qsspecl_then [‘g o p1(A,1)’] assume_tac Ev_of_Tp >> rfs[]) >>
  rw[GSYM Tp1_def] >> irule is_Tp >>
  arw[o_assoc] >> rw[GSYM o_assoc] >>
- qsspecl_then [‘f’] assume_tac Ev_of_Tp >> rfs[] >>
- irule o_Fun >> arw[])
+ qsspecl_then [‘f’] assume_tac Ev_of_Tp >> rfs[])
 (form_goal
- “!A B f: A * N ~>B g:A~>B. isFun(f) & isFun(g) ==>
+ “!A B f: A * N ->B g:A->B.
   (Tp(f) o El(O) = Tp1(g) <=> f o Pa(p1(A,1),El(O) o p2(A,1)) = g o p1(A,1))”));
 
 
 
 val Pa_p1_p2 = prove_store("Pa_p1_p2",
 e0
-(rpt strip_tac >>
- fconv_tac (rewr_fconv (eq_sym "rel")) >>
- irule is_Pa >> rw[idR,p12_Fun,id_Fun])
+(rpt strip_tac >> flip_tac >> irule is_Pa >> rw[IdR])
 (form_goal
- “!A B. Pa(p1(A,B),p2(A,B)) = id(A * B)”));
-
-
+ “!A B. Pa(p1(A,B),p2(A,B)) = Id(A * B)”));
 
 
 val Thm1_comm_eq_right = prove_store("Thm1_comm_eq_right",
 e0
 (rpt strip_tac >>
- qspecl_then [‘A’,‘N * Exp(A,B)’] assume_tac p12_Fun >>
- qspecl_then [‘A * N’] assume_tac id_Fun >>
- assume_tac SUC_Fun >>
- qspecl_then [‘A’,‘N’] assume_tac p12_Fun >>
- qspecl_then [‘N’,‘Exp(A,B)’] assume_tac p12_Fun >>
- qspecl_then [‘A’,‘B’] assume_tac Ev_Fun >>
- qsspecl_then [‘f’] assume_tac Tp_Fun >> rfs[] >>
- qsspecl_then [‘p2(A,N)’,‘SUC’] assume_tac o_Fun >> rfs[] >>
- qsspecl_then [‘p1(A,N)’,‘SUC o p2(A,N)’] assume_tac Pa_Fun >> rfs[] >>
- qsspecl_then [‘id(A * N)’,‘f’] assume_tac Pa_Fun >> rfs[] >>
- qspecl_then [‘N’] assume_tac id_Fun >> 
- qsspecl_then [‘id(N)’,‘Tp(f)’] assume_tac Pa_Fun >> rfs[] >>
- qsspecl_then [‘Pa(id(A * N),f)’,‘h’] assume_tac o_Fun >> rfs[] >>
- qsspecl_then [‘Pa(p1(A, N), SUC o p2(A, N))’,‘f’] assume_tac o_Fun >>
- rfs[] >> 
- qsspecl_then [‘SUC’,‘Tp(f)’] assume_tac o_Fun >> rfs[] >>
- qsspecl_then [‘p2(A, N * Exp(A, B))’,‘p2(N, Exp(A, B))’] 
- assume_tac o_Fun >> rfs[] >>
- qsspecl_then [‘p1(A, N * Exp(A, B))’,‘p2(N, Exp(A, B)) o
-                 p2(A, N * Exp(A, B))’] assume_tac Pa_Fun >> rfs[] >>
- qsspecl_then [‘Pa(p1(A, N * Exp(A, B)), p2(N, Exp(A, B)) o
-                 p2(A, N * Exp(A, B)))’,‘Ev(A,B)’] assume_tac o_Fun >>
- rfs[] >> 
- qsspecl_then [‘p2(A, N * Exp(A, B))’,‘p1(N, Exp(A, B))’]
- assume_tac o_Fun >> rfs[] >>
- qsspecl_then [‘p1(A, N * Exp(A, B))’,‘p1(N, Exp(A, B)) o p2(A, N * Exp(A, B))’] assume_tac Pa_Fun >> rfs[] >>
- qsspecl_then [‘Pa(p1(A, N * Exp(A, B)), p1(N, Exp(A, B)) o p2(A, N * Exp(A, B)))’,‘Ev(A, B) o
-                Pa(p1(A, N * Exp(A, B)), p2(N, Exp(A, B)) o
-                 p2(A, N * Exp(A, B)))’] assume_tac Pa_Fun >> rfs[] >>
- qsspecl_then [‘l’,‘h’] assume_tac o_Fun >> rfs[] >>
- qsspecl_then [‘h o l’] assume_tac Tp_Fun >> rfs[] >>
- qsspecl_then [‘Pa(id(N), Tp(f))’,‘Tp(h o l)’] assume_tac o_Fun >> rfs[] >>
  qsuff_tac
- ‘Tp(h o l) o Pa(id(N),Tp(f)) = Tp(h o Pa(id(A * N),f)) & 
+ ‘Tp(h o l) o Pa(Id(N),Tp(f)) = Tp(h o Pa(Id(A * N),f)) & 
   Tp(f o Pa(p1(A,N), SUC o p2(A,N))) = Tp(f) o SUC’
  >-- (strip_tac >> dimp_tac >> strip_tac (* 2 *)
       >-- arw[] >>
       irule $ iffLR Tp_eq >> arw[] >>
       qpick_x_assum
-      ‘Tp((h o l)) o Pa(id(N), Tp(f)) =
-       Tp(h o Pa(id(A * N), f))’
+      ‘Tp((h o l)) o Pa(Id(N), Tp(f)) =
+       Tp(h o Pa(Id(A * N), f))’
       (assume_tac o GSYM) >> arw[]) >>
  strip_tac (* 2 *) >--
  (irule is_Tp >> 
-  qby_tac
-  ‘Pa(p1(A, N), (Tp((h o l)) o Pa(id(N), Tp(f))) o p2(A, N))=
-   Pa(p1(A,N * Exp(A,B)), Tp(h o l) o p2(A,N * Exp(A,B))) o 
-   Pa(p1(A,N),Pa(id(N),Tp(f)) o p2(A,N))’ >-- 
-  (rw[o_assoc] >> irule Pa_o_split >> arw[]) >>
+        qby_tac
+        ‘Pa(p1(A, N), (Tp((h o l)) o Pa(Id(N), Tp(f))) o p2(A, N))=
+  Pa(p1(A,N * Exp(A,B)), Tp(h o l) o p2(A,N * Exp(A,B))) o 
+  Pa(p1(A,N),Pa(Id(N),Tp(f)) o p2(A,N))’ >-- 
+  rw[o_assoc,Pa_o_split] >> 
   once_arw[] >> rw[GSYM o_assoc] >>
   qsspecl_then [‘h o l’] assume_tac Ev_of_Tp >> rfs[] >>
   rw[o_assoc] >> 
-  qsspecl_then [‘p2(A,N)’,‘Pa(id(N), Tp(f))’] assume_tac o_Fun >> rfs[] >>
-  qsspecl_then [‘p1(A,N)’,‘Pa(id(N), Tp(f)) o p2(A, N)’] 
-  assume_tac Pa_Fun >> rfs[] >>
-  qsspecl_then [‘Pa(p1(A, N), Pa(id(N), Tp(f)) o p2(A, N))’,‘l’] 
-  assume_tac o_Fun >> rfs[] >>
   qsuff_tac
-  ‘l o Pa(p1(A, N), Pa(id(N), Tp(f)) o p2(A, N)) = 
-   Pa(id(A * N), f)’ >--
+  ‘l o Pa(p1(A, N), Pa(Id(N), Tp(f)) o p2(A, N)) = 
+   Pa(Id(A * N), f)’ >--
   (strip_tac >> arw[]) >>
   irule to_P_eq >> arw[] >> 
-  qsspecl_then [‘id(A * N)’,‘f’] assume_tac p12_of_Pa >> rfs[] >>
   qpick_x_assum
   ‘Pa(Pa(p1(A, N * Exp(A, B)), p1(N, Exp(A, B)) o p2(A, N * Exp(A, B))),
                 Ev(A, B) o
@@ -647,78 +451,93 @@ e0
                  p2(A, N * Exp(A, B)))) = l’
   (assume_tac o GSYM) >> arw[] >>
   rw[GSYM o_assoc] >>
-  qsspecl_then [‘Pa(p1(A, N * Exp(A, B)), p1(N, Exp(A, B)) o
-                 p2(A, N * Exp(A, B)))’,‘Ev(A, B) o
-                Pa(p1(A, N * Exp(A, B)), p2(N, Exp(A, B)) o
-                 p2(A, N * Exp(A, B)))’] assume_tac p12_of_Pa >>
-  rfs[] >>
-  qsspecl_then [‘p1(A, N * Exp(A, B))’,‘p1(N, Exp(A, B)) o
-                p2(A, N * Exp(A, B))’,‘Pa(p1(A, N), Pa(id(N), Tp(f)) o p2(A, N))’] assume_tac Pa_distr' >> rfs[] >>
-  qsspecl_then [‘p1(A, N)’,‘Pa(id(N), Tp(f)) o p2(A, N)’]
-  assume_tac p12_of_Pa >> rfs[] >>
-  fs[o_assoc] >>
-  rw[GSYM o_assoc] >>
-  qsspecl_then [‘id(N)’,‘Tp(f)’] assume_tac p12_of_Pa >> rfs[] >>
-  rw[idL,Pa_p1_p2] >>
-  fs[o_assoc] >>
-  qsspecl_then [‘p1(A, N * Exp(A, B))’,‘p2(N, Exp(A, B)) o
-                p2(A, N * Exp(A, B))’,‘Pa(p1(A, N), Pa(id(N), Tp(f)) o p2(A, N))’] assume_tac Pa_distr' >>
-  rfs[] >>fs[o_assoc] >> fs[GSYM o_assoc] >> 
-  qsspecl_then [‘f’] assume_tac Ev_of_Tp >> rfs[]) >>
- (*flip tac does not work here*) 
- fconv_tac (rewr_fconv (eq_sym "rel"))  >> irule is_Tp >> arw[] >> 
+  rw[p12_of_Pa,Pa_distr,o_assoc,Ev_of_Tp,IdL,Pa_p1_p2]) >>
+ flip_tac >> irule is_Tp >> arw[] >> 
  qby_tac
  ‘Pa(p1(A, N), (Tp(f) o SUC) o p2(A, N)) = 
   Pa(p1(A, N), Tp(f) o p2(A,N)) o Pa(p1(A,N),SUC o p2(A,N))’
- >-- (rw[o_assoc] >> irule Pa_o_split >> arw[]) >>
+ >-- rw[o_assoc,Pa_o_split] >>
  arw[GSYM o_assoc] >> 
  qsspecl_then [‘f’] assume_tac Ev_of_Tp >> rfs[]
  )
 (form_goal
- “!A B f:A * N ~>B h: (A * N) * B ~>B. isFun(f) & isFun(h) ==> !l . 
+ “!A B f:A * N ->B h: (A * N) * B ->B. !l . 
 Pa(
  Pa(p1(A,N * Exp(A,B)), p1(N,Exp(A,B)) o p2(A,N * Exp(A,B))),
  Ev(A,B) o 
  Pa(p1(A,N * Exp(A,B)), p2(N,Exp(A,B)) o p2(A,N * Exp(A,B)))) = l
  ==>
- (h o Pa(id(A * N),f) = f o Pa(p1(A,N), SUC o p2(A,N)) <=>
- Tp(h o l) o Pa(id(N),Tp(f)) = Tp(f) o SUC)”));
+ (h o Pa(Id(A * N),f) = f o Pa(p1(A,N), SUC o p2(A,N)) <=>
+ Tp(h o l) o Pa(Id(N),Tp(f)) = Tp(f) o SUC)”));
 
 
-val Thm1_comm_eq_condition = prove_store(
-"Thm1_comm_eq_condition",
+val Ev_of_Tp_el = prove_store("Ev_of_Tp_el",
+e0
+(rpt strip_tac >>
+ assume_tac Ev_of_Tp >> 
+ first_x_assum (qspecl_then [‘A’,‘B’,‘X’,‘f’] assume_tac) >>
+ qby_tac 
+ ‘Pa(a, Tp(f) o x) = Pa(p1(A, X), Tp(f) o p2(A, X)) o Pa(a,x)’ >--
+ (irule to_P_eq >> rw[p12_of_Pa] >> 
+  rw[p12_of_Pa,GSYM o_assoc] >> rw[o_assoc,p12_of_Pa]) >>
+ arw[GSYM o_assoc])
+(form_goal
+ “!A B X f:A * X ->B P a:P->A x: P ->X. 
+  Ev(A,B) o Pa(a, Tp(f) o x) = f o Pa(a,x)”));
+
+
+
+val Ev_of_Tp_el' = prove_store("Ev_of_Tp_el'",
 e0
 (rpt strip_tac >> 
- qsspecl_then [‘f’,‘h’] assume_tac Thm1_comm_eq_right >> rfs[] >>
- first_x_assum drule >> 
- qsspecl_then [‘f’,‘g’] (assume_tac o GSYM) Thm1_comm_eq_left >> rfs[])
+ qby_tac ‘Tp(f) = Tp(f) o Id(P)’ >-- rw[IdR] >>
+ once_arw[] >> rw[Ev_of_Tp_el])
 (form_goal
- “!A B f: A * N ~>B g:A~>B h: (A * N) * B ~> B. isFun(f) & isFun(h) & isFun(g) ==>
- !l.
- Pa(
- Pa(p1(A,N * Exp(A,B)), p1(N,Exp(A,B)) o p2(A,N * Exp(A,B))),
- Ev(A,B) o 
- Pa(p1(A,N * Exp(A,B)), p2(N,Exp(A,B)) o p2(A,N * Exp(A,B)))) = l ==>
- (f o Pa(p1(A,1),El(O) o p2(A,1)) = g o p1(A,1) & 
-  h o Pa(id(A * N),f) = f o Pa(p1(A,N), SUC o p2(A,N)) <=>
-  Tp(f) o El(O) = Tp1(g) & Tp(h o l) o Pa(id(N),Tp(f)) = Tp(f) o SUC)
-  ”));
+“!A B P f:A * P -> B  a:P -> A.
+Ev(A, B) o Pa(a, Tp(f)) = f o Pa(a, Id(P))”));
 
-*)
 
-val Thm1_case_1 = prove_store("Thm1_case_1",
+val Tp_of_Ev = prove_store("Tp_of_Ev",
 e0
-cheat
+(flip_tac >> irule is_Tp >> rw[])
 (form_goal
- “!B g:1->B h:N * B -> B. 
- ?!f:N->B.  f o El(O) = g & f o SUC = h o Pa(Id(N),f)”));
-
-
+ “Tp((Ev(A, B) o Pa(p1(A, X), f o p2(A, X)))) = f”));
 
 
 val Thm1 = prove_store("Thm1",
 e0
-cheat
+(rpt strip_tac >>
+ abbrev_tac “Tp(g:A->B o p1(A,1)) = g'” >>
+ abbrev_tac “Pa(
+ Pa(p1(A,N * Exp(A,B)), p1(N,Exp(A,B)) o p2(A,N * Exp(A,B))),
+ Ev(A,B) o 
+ Pa(p1(A,N * Exp(A,B)), p2(N,Exp(A,B)) o p2(A,N * Exp(A,B)))) = l” >>
+ abbrev_tac “Tp(h:(A * N) * B->B o l:A * N * Exp(A,B) -> (A * N) * B) = h'” >>
+ qspecl_then [‘Exp(A,B)’,‘g'’,‘h'’] assume_tac Thm1_case_1 >>
+ pop_assum (assume_tac o uex_expand) >>
+ pop_assum (x_choose_then "fb" assume_tac) >> 
+ qexists_tac ‘Ev(A,B) o Pa(p1(A,N),fb o p2(A,N)) ’ >>
+ rw[GSYM Thm1_comm_eq_left] >>
+ qspecl_then [‘A’,‘B’,‘Ev(A,B) o Pa(p1(A,N),fb o p2(A,N))’] assume_tac
+ Thm1_comm_eq_right >> first_x_assum drule >>
+ rpt strip_tac >> dimp_tac >> strip_tac >--
+ (qspecl_then [‘A’,‘B’,‘f0’] assume_tac 
+ Thm1_comm_eq_right >> first_x_assum drule >> rfs[] >>
+ qsuff_tac ‘fb = Tp(f0)’ 
+ >-- (strip_tac >> arw[Ev_of_Tp]) >>
+ qsspecl_then [‘g'’,‘h'’] assume_tac Thm1_case_1 >>
+ pop_assum (assume_tac o uex_expand) >> 
+ pop_assum strip_assume_tac >>
+ qsuff_tac ‘fb = f & Tp(f0 ) = f’
+ >-- (strip_tac >> arw[]) >>
+ strip_tac >> first_x_assum irule >> arw[GSYM Tp1_def]) >> 
+ once_arw[] >> strip_tac (* 2 *)
+ >-- (rw[GSYM Tp1_def] >> irule is_Tp >> 
+ rw[Pa_o_split,o_assoc,Ev_of_Tp_el] >>
+ rw[Pa_o_split,GSYM o_assoc,Ev_of_Tp_el] >>
+ rw[o_assoc,p12_of_Pa,Pa_distr] >> irule $ iffLR Tp_eq >>
+ flip_tac >> arw[GSYM o_assoc] >> irule is_Tp >> rw[]) >>
+ first_x_assum $ irule o iffRL >> rw[Tp_of_Ev] >> arw[])
 (form_goal
  “!A B g:A->B h:(A * N) * B ->B. 
  ?f:A * N ->B. !f0.
@@ -729,258 +548,89 @@ val PRE_def0 =
     Thm1_case_1 |> specl (List.map rastt ["N","El(O)","p1(N,N)"])
                 |> uex_expand 
                 |> qSKOLEM "PRE" []
-                |> 
-
-val PRE_def0 = PRE_ex |> ex2fsym0 "PRE" []
-                     |> store_as "PRE_def0";
 
 
 val Pre_def = qdefine_fsym ("Pre",[‘n:mem(N)’]) ‘App(PRE,n)’ 
                            |> gen_all |> store_as "Pre_def";
 
-(*
+
 val PRE_def = prove_store("PRE_def",
 e0
-(assume_tac PRE_def0 >> 
- qspecl_then [‘N’] assume_tac id_Fun>>
- qsspecl_then [‘id(N)’,‘PRE’] assume_tac Pa_Fun >> rfs[] >> 
- irule p1_of_Pa >> arw[]
- )
+(assume_tac PRE_def0 >> fs[p12_of_Pa])
 (form_goal
- “ PRE o El(O) = El(O) & PRE o SUC = id(N) &
- !f:N~>N.
-  isFun(f) &
-  f o El(O) = El(O) & f o SUC = p1(N, N) o Pa(id(N), f) ==> f = PRE”));
+ “ PRE o El(O) = El(O) & PRE o SUC = Id(N)”));
 
-val PRE_Fun = PRE_def |> conjE1 |> store_as "PRE_Fun";
 
-val Pre_ex = prove_store("Pre_ex",
+val Pre_eqn = prove_store("Pre_eqn",
 e0
-(strip_tac >> qexists_tac ‘App(PRE,n)’ >> rw[])
-(form_goal
- “!n. ?pn. App(PRE,n) = pn”));
-
-val Pre_def = Pre_ex |> spec_all |> ex2fsym0 "Pre" ["n"]
-                     |> store_as "Pre_def";
-
-val Suc_ex = prove_store("Suc_ex",
-e0
-(strip_tac >> qexists_tac ‘App(SUC,n)’ >> rw[])
-(form_goal
- “!n.?sn. App(SUC,n) = sn”));
-
-val Suc_def = Suc_ex |> spec_all |> ex2fsym0 "Suc" ["n"]
-
-
-val lflip_tac = fconv_tac (land_fconv no_conv (once_depth_fconv no_conv (rewr_fconv (eq_sym "mem"))))
-
-(*lflip does not work...*)
-
-val O_xor_Suc = prove_store("O_xor_Suc",
-e0
-(rw[O_xor_SUC,GSYM Suc_def] >> strip_tac >> dimp_tac >> strip_tac >>
- qexists_tac ‘pn’ >> arw[])
-(form_goal
- “!n. ~(n = O) <=> ?pn. n = Suc(pn)”));
-
-val Suc_eq_eq = prove_store("Suc_eq_eq",
-e0
-(assume_tac SUC_eq_eq >> fs[Suc_def])
-(form_goal
- “!m n.Suc(m) = Suc(n) <=> m = n”));
-
-val Pre_eqn = prove_store("PRE_eqn",
-e0
-(strip_assume_tac PRE_def >> pop_assum (K all_tac) >>
+(strip_assume_tac PRE_def >> 
  qby_tac
  ‘App(PRE o El(O),dot) = App(El(O),dot)’ 
  >-- arw[] >> fs[El_def] >>
- qsspecl_then [‘El(O)’,‘PRE’,‘dot’] assume_tac $ GSYM o_App >>
- qsspecl_then [‘O’] assume_tac El_Fun >>
- assume_tac PRE_Fun >> fs[] >> fs[El_def] >> arw[GSYM Pre_def] >>
- strip_tac >>
- qby_tac ‘App(PRE o SUC,n) = App(id(N),n)’ 
+ fs[App_App_o,El_def,Pre_def] >> strip_tac >>
+ qby_tac ‘App(PRE o SUC,n) = App(Id(N),n)’ 
  >-- arw[] >>
- qsspecl_then [‘SUC’,‘PRE’,‘n’] assume_tac o_App >>
- assume_tac SUC_Fun >> fs[] >> rfs[] >>
- fs[GSYM Suc_def,App_id])
+ fs[App_App_o,Pre_def,Suc_def,Id_def])
 (form_goal
  “Pre(O) = O & !n. Pre(Suc(n)) = n”));
-*)
 
 
-val ADD_def0 = 
+
+val ADD_def = 
  Thm1 |> sspecl (List.map rastt ["Id(N)","SUC o p2(N * N,N)"])
       |> qSKOLEM "ADD" []
-      |> store_as "ADD_def0";
+      |> rewr_rule[o_assoc,p12_of_Pa,IdL]
+      |> qspec ‘ADD’ |> rewr_rule[To1_def]
+      |> store_as "ADD_def";
         
-(*
-val ADD_def0 = ADD_ex |> ex2fsym0 "ADD" []
-                      |> store_as "ADD_def0";
-
-val is_To1 = To1_def |> spec_all |> conjE2 |> gen_all
-                     |> store_as "is_To1";
-
-val To1_Fun = To1_def |> spec_all |> conjE1 |> gen_all
-                     |> store_as "To1_Fun";
-
-val ADD_property = prove_store("ADD_property",
-e0
-(assume_tac ADD_def0 >> 
- first_x_assum $ qspecl_then [‘ADD’] assume_tac >> fs[idL] >>
- qby_tac ‘p2(N,1) = To1(N * 1)’
- >-- (qspecl_then [‘N’,‘1’] assume_tac p12_Fun >> fs[] >>
-     drule is_To1 >> arw[]) >>
- fs[o_assoc] >> 
- qby_tac
- ‘ADD o Pa(p1(N, 1), El(O) o To1(N * 1)) o Pa(id(N),To1(N)) = p1(N, 1) o Pa(id(N),To1(N))’
- >-- arw[GSYM o_assoc] >>
- qsspecl_then [‘id(N)’,‘To1(N)’] assume_tac p1_of_Pa >>
- fs[id_Fun,To1_Fun] >>
- qsspecl_then [‘p1(N,1)’,‘El(O) o To1(N * 1)’,‘Pa(id(N),To1(N))’]
- assume_tac $ Pa_distr' >>
- qspecl_then [‘N’] assume_tac id_Fun >>
- qspecl_then [‘N’] assume_tac To1_Fun >>
- qsspecl_then [‘id(N)’,‘To1(N)’] assume_tac Pa_Fun >> rfs[] >>
- qspecl_then [‘N * 1’] assume_tac To1_Fun>>
- qsspecl_then [‘O’] assume_tac El_Fun >>
- qsspecl_then [‘To1(N * 1)’,‘El(O)’] assume_tac o_Fun >> rfs[] >>
- qspecl_then [‘N’,‘1’] assume_tac p12_Fun >> fs[] >>
- fs[o_assoc] >>
- qsspecl_then [‘To1(N * 1) o Pa(id(N), To1(N))’] assume_tac is_To1 >>
- qby_tac ‘isFun(To1(N * 1) o Pa(id(N), To1(N)))’
- >-- (irule o_Fun >> rw[To1_Fun] >> irule Pa_Fun >> rw[To1_Fun,id_Fun])>>
- fs[])
-(form_goal
- “isFun(ADD) & 
-  ADD o Pa(id(N),El(O) o To1(N)) = id(N) & 
- ADD o Pa(p1(N,N),SUC o p2(N,N)) = SUC o p2(N * N,N) o Pa(id(N * N),ADD)”));
-
-
-val ADD_Fun = ADD_property |> conjE1 |> store_as "ADD_Fun";
-
-val ADD_El0 = ADD_property |> conjE2 |> store_as "ADD_El0";
-
-val ADD_El = prove_store("ADD_El",
-e0
-(assume_tac ADD_property >> arw[] >>
- qsspecl_then [‘id(N * N)’,‘ADD’] assume_tac p2_of_Pa >>
- fs[id_Fun,ADD_Fun])
-(form_goal
- “ADD o Pa(id(N),El(O) o To1(N)) = id(N) & 
-  ADD o Pa(p1(N,N),SUC o p2(N,N)) = SUC o ADD”));
-*)
 
 val Add_def = qdefine_fsym ("Add",[‘n1:mem(N)’,‘n2:mem(N)’]) ‘App(ADD,Pair(n1,n2))’ |> gen_all |> store_as "Add_def";
 
-(*
-val Add_ex = prove_store("Add_ex",
-e0
-(rpt strip_tac >> qexists_tac ‘App(ADD,Pair(m,n))’ >> rw[])
-(form_goal
- “!m n. ?amn. App(ADD,Pair(m,n)) = amn”));
-
-val Add_def = Add_ex |> spec_all |> ex2fsym0 "Add" ["m","n"] 
-                     |> gen_all |> store_as "Add_def";
 
 val App_input_eq =prove_store("App_input_eq",
 e0
 (rpt strip_tac >> arw[])
 (form_goal
- “!A B f:A~>B a1 a2.a1 = a2 ==> App(f,a1) = App(f,a2)”))
+ “!A B f:A->B a1 a2.a1 = a2 ==> App(f,a1) = App(f,a2)”))
 
-val App_Pa_Pair = prove_store("App_Pa_Pair",
-e0
-(rpt strip_tac >>  irule Cross_eq >> rw[Pair_def] >> strip_tac >>
- irule $ iffLR App_o_l >> 
- qsspecl_then [‘f’,‘g’] assume_tac p12_of_Pa >> rfs[] >>
- rw[p12_Fun] >> irule Pa_Fun >> arw[])
-(form_goal
- “!X A f:X~>A B g:X~>B. isFun(f) & isFun(g) ==>
-  !x:mem(X).App(Pa(f,g),x) = Pair(App(f,x),App(g,x))”));
-
-(* (∀n. 0 + n = n) ∧ ∀m n. SUC m + n = SUC (m + n)*)
-val Add_O = prove_store("Add_O",
-e0
-(strip_tac >> fs[GSYM Add_def] >>
- assume_tac ADD_El >>
- qsuff_tac ‘App(ADD o Pa(id(N), El(O) o To1(N)),n) = App(ADD, Pair(n, O)) & App(id(N),n) = n’
- >-- (strip_tac >>rfs[]) >>
- rw[App_id] >> irule $iffRL App_o_l >> rw[ADD_Fun] >>
- qspecl_then [‘N’] assume_tac id_Fun >>
- qspecl_then [‘N’] assume_tac To1_Fun >>
- qsspecl_then [‘To1(N)’,‘El(O)’] assume_tac o_Fun >> rfs[] >>
- qsspecl_then [‘O’] assume_tac El_Fun >> fs[] >>
- qsspecl_then [‘id(N)’,‘El(O) o To1(N)’] assume_tac Pa_Fun >> rfs[] >>
- irule App_input_eq >> 
- (*irule with eval_pa does not work, some sort of irule at?*)
- qsspecl_then [‘id(N)’,‘El(O) o To1(N)’] assume_tac App_Pa_Pair >>
- rfs[] >> fs[App_id] >>
- rw[Pair_eq_eq] >> irule $ iffRL App_o_l >> arw[] >> rw[dot_def] >>
- rw[App_El])
-(form_goal
- “!n. Add(n,O) = n”));
-
+val App_Pa_Pair = App_Pa_distr |> store_as "App_Pa_Pair";
 
 
 (* (∀n. 0 + n = n) ∧ ∀m n. SUC m + n = SUC (m + n)*)
 val Add_O = prove_store("Add_O",
 e0
-(strip_tac >> fs[GSYM Add_def] >>
- assume_tac ADD_El >>
- qsuff_tac ‘App(ADD o Pa(id(N), El(O) o To1(N)),n) = App(ADD, Pair(n, O)) & App(id(N),n) = n’
- >-- (strip_tac >>rfs[]) >>
- rw[App_id] >> irule $iffRL App_o_l >> rw[ADD_Fun] >>
- qspecl_then [‘N’] assume_tac id_Fun >>
- qspecl_then [‘N’] assume_tac To1_Fun >>
- qsspecl_then [‘To1(N)’,‘El(O)’] assume_tac o_Fun >> rfs[] >>
- qsspecl_then [‘O’] assume_tac El_Fun >> fs[] >>
- qsspecl_then [‘id(N)’,‘El(O) o To1(N)’] assume_tac Pa_Fun >> rfs[] >>
- irule App_input_eq >> 
- (*irule with eval_pa does not work, some sort of irule at?*)
- qsspecl_then [‘id(N)’,‘El(O) o To1(N)’] assume_tac App_Pa_Pair >>
- rfs[] >> fs[App_id] >>
- rw[Pair_eq_eq] >> irule $ iffRL App_o_l >> arw[] >> rw[dot_def] >>
- rw[App_El])
+(strip_tac >> 
+ assume_tac ADD_def >>
+ qby_tac ‘App(ADD o Pa(p1(N, 1), El(O) o To1(N * 1)),Pair(n,dot)) = 
+  App(p1(N, 1),Pair(n,dot))’
+ >-- arw[] >>
+ pop_assum mp_tac >> 
+ rw[p12_of_Pair,App_App_o,App_Pa_distr,dot_def,El_def,Add_def])
 (form_goal
  “!n. Add(n,O) = n”));
 
 
 val Add_Suc = prove_store("Add_Suc",
 e0
-(rpt strip_tac >> assume_tac ADD_El >> fs[] >> last_x_assum (K all_tac) >>
- rw[GSYM Add_def,GSYM Suc_def] >>
- flip_tac >> irule $ iffLR App_o_l >> pop_assum (assume_tac o GSYM) >>
- arw[] >> rw[ADD_Fun,SUC_Fun] >> irule $ iffRL App_o_l >> 
- rw[ADD_Fun] >>
- qspecl_then [‘N’,‘N’] assume_tac p12_Fun >>
- qsspecl_then [‘p2(N,N)’,‘SUC’] assume_tac o_Fun >> rfs[] >>
- assume_tac SUC_Fun >> fs[] >>
- qsspecl_then [‘p1(N,N)’,‘SUC o p2(N,N)’] assume_tac Pa_Fun >>
- rfs[] >> irule App_input_eq >> 
- qsspecl_then [‘p1(N,N)’,‘SUC o p2(N,N)’] assume_tac App_Pa_Pair >>
- rfs[] >> rw[Pair_def] >> rw[Pair_eq_eq] >> 
- irule $ iffRL App_o_l >> arw[] >> irule App_input_eq >>
- rw[Pair_def])
+(rpt strip_tac >> assume_tac ADD_def >>
+ qby_tac ‘App(SUC o ADD,Pair(m,n)) =
+          App(ADD o Pa(p1(N, N), SUC o p2(N, N)),Pair(m,n))’
+ >-- arw[] >>
+ pop_assum mp_tac >> rw[App_App_o,App_Pa_distr,p12_of_Pair,Suc_def,Add_def] >>
+ strip_tac >> arw[])
 (form_goal
  “(!m n.Add(m,Suc(n)) = Suc(Add(m,n)))”));
 
 val Pre_O = conjE1 Pre_eqn |> store_as "Pre_O";
 
 val Pre_Suc = conjE2 Pre_eqn |> store_as "Pre_Suc";
-*)
 
 
-val SUB_def0 = Thm1 |> specl
+val SUB_def = Thm1 |> specl
 (List.map rastt ["N","N","Id(N)","PRE o p2(N * N,N)"])
 |> qSKOLEM "SUB" []
-|> store_as "SUB_def0";
-
-(*
-val SUB_def0' = SUB_def0 |> specl [rastt "SUB"] |> rewr_rule[]
-
-val SUB_Fun = SUB_def0' |> conjE1 |> store_as "SUB_Fun";
-
+|> qspec ‘SUB’ |> rewr_rule[IdL,o_assoc,p12_of_Pa]
+|> store_as "SUB_def";
 
 
 
@@ -988,92 +638,40 @@ val o_eq_r = prove_store("o_eq_r",
 e0
 (rpt strip_tac >> arw[])
 (form_goal
- “!A B f1:A~>B f2:A~>B. f1 = f2 ==>
-  !C g:B~>C. g o f1 = g o f2”));
+ “!A B f1:A->B f2:A->B. f1 = f2 ==>
+  !C g:B->C. g o f1 = g o f2”));
 
-
-val SUB_El = prove_store("SUB_El",
-e0
-(strip_assume_tac SUB_def0' >> 
- qby_tac
- ‘SUB o Pa(p1(N, 1), El(O) o p2(N, 1)) o Pa(id(N),To1(N)) = p1(N, 1) o Pa(id(N),To1(N))’
- >-- arw[GSYM o_assoc] >>
- qspecl_then [‘N’] assume_tac id_Fun >>
- qspecl_then [‘N’] assume_tac To1_Fun >>
- qsspecl_then [‘id(N)’,‘To1(N)’] assume_tac Pa_Fun >> rfs[] >>
- qsspecl_then [‘id(N)’,‘To1(N)’] assume_tac p1_of_Pa >> rfs[] >>
- fs[] >> 
- qsspecl_then [‘O’] assume_tac El_Fun >>
- qspecl_then [‘N’,‘1’] assume_tac p12_Fun >>
- qsspecl_then [‘p2(N,1)’,‘El(O)’] assume_tac o_Fun >> rfs[] >>
- qsspecl_then [‘p1(N,1)’,‘El(O) o p2(N,1)’,‘Pa(id(N),To1(N))’] assume_tac
- Pa_distr' >> rfs[] >> fs[] >> fs[o_assoc] >>
- qsspecl_then [‘id(N)’,‘To1(N)’] assume_tac p2_of_Pa >> rfs[] >> fs[] >> 
- qpick_x_assum 
- ‘PRE o p2(N * N, N) o Pa(id(N * N), SUB) = SUB o Pa(p1(N, N), SUC o p2(N, N))’ (assume_tac o GSYM) >>
- arw[] >> irule o_eq_r >>
- qsspecl_then [‘id(N * N)’,‘SUB’] assume_tac p2_of_Pa >> rfs[id_Fun])
-(form_goal
- “SUB o Pa(id(N), El(O) o To1(N)) = id(N) &
- PRE o SUB = SUB o Pa(p1(N,N), SUC o p2(N,N))”));
-*)
 
 val Sub_def = qdefine_fsym ("Sub",[‘n1:mem(N)’,‘n2:mem(N)’]) ‘App(SUB,Pair(n1,n2))’ |> gen_all |> store_as "Sub_def";
 
 
-(*
-val Sub_ex = prove_store("Sub_ex",
-e0
-(rpt strip_tac >> qexists_tac ‘App(SUB,Pair(m,n))’ >> rw[])
-(form_goal
- “!m n.?smn. App(SUB,Pair(m,n)) = smn”));
-
-val Sub_def = Sub_ex |> spec_all |> ex2fsym0 "Sub" ["m","n"] 
-                     |> gen_all |> store_as "Sub_def";
 
 val Sub_O = prove_store("Sub_O",
 e0
-(strip_tac >> strip_assume_tac SUB_El >>
- pop_assum (K all_tac) >>
- qby_tac
- ‘App(SUB o Pa(id(N), El(O) o To1(N)),n) = App(id(N),n)’ 
- >-- arw[] >>
- fs[App_id] >> fs[GSYM Sub_def] >> 
- qsuff_tac
- ‘App(SUB o Pa(id(N), El(O) o To1(N)), n) = App(SUB, Pair(n, O))’ 
- >-- (strip_tac >> fs[]) >>
- irule $ iffRL App_o_l >> rw[SUB_Fun] >>
- qsspecl_then [‘O’] assume_tac El_Fun >> 
- qspecl_then [‘N’] assume_tac To1_Fun >> 
- qsspecl_then [‘To1(N)’,‘El(O)’] assume_tac o_Fun >> rfs[] >>
- qspecl_then [‘N’] assume_tac id_Fun >>
- qsspecl_then [‘id(N)’,‘El(O) o To1(N)’] assume_tac Pa_Fun >>
- rfs[] >> irule App_input_eq >>
- qsspecl_then [‘id(N)’,‘El(O) o To1(N)’] assume_tac App_Pa_Pair >>
- rfs[] >> rw[Pair_eq_eq] >> irule $ iffRL App_o_l >>
- arw[] >> rw[dot_def,El_def]
- )
+(strip_tac >> strip_assume_tac SUB_def >>
+ qby_tac 
+ ‘App(SUB o Pa(p1(N, 1), El(O) o p2(N, 1)),Pair(n,dot)) = 
+      App(p1(N, 1),Pair(n,dot))’
+ >-- arw[] >> 
+ pop_assum mp_tac >>
+ rw[App_App_o,p12_of_Pair,App_Pa_distr,El_def,Sub_def])
 (form_goal
  “!n. Sub(n,O) = n”));
 
 
 val Sub_Suc = prove_store("Sub_Suc",
 e0
-(rpt strip_tac >> strip_assume_tac SUB_El >> last_x_assum (K all_tac) >>
- rw[GSYM Sub_def,GSYM Suc_def,GSYM Pre_def] >> 
- flip_tac >> irule $ iffLR App_o_l >> arw[] >>
- rw[PRE_Fun,SUB_Fun] >> 
- irule $ iffRL App_o_l >> rw[SUB_Fun] >>
- qspecl_then [‘N’,‘N’] assume_tac p12_Fun >>
- assume_tac SUC_Fun >>
- qsspecl_then [‘p2(N,N)’,‘SUC’] assume_tac o_Fun >> rfs[] >>
- qsspecl_then [‘p1(N,N)’,‘SUC o p2(N,N)’] assume_tac Pa_Fun >> rfs[] >>
- irule App_input_eq >> 
- qsspecl_then [‘p1(N,N)’,‘SUC o p2(N,N)’] assume_tac App_Pa_Pair >> 
- rfs[] >> rw[Pair_eq_eq] >> rw[Pair_def] >> irule $ iffRL App_o_l >>
- arw[] >> irule App_input_eq >> rw[Pair_def])
+(rpt strip_tac >> strip_assume_tac SUB_def >> 
+ qby_tac
+ ‘App(PRE o SUB,Pair(m,n)) =
+  App(SUB o Pa(p1(N, N), SUC o p2(N, N)),Pair(m,n))’ 
+ >-- arw[] >> pop_assum mp_tac >>
+ rw[App_App_o,App_App_o,p12_of_Pair,App_Pa_distr,Pre_def,Sub_def,Suc_def] >>
+ strip_tac >> arw[])
 (form_goal
  “!m n. Sub(m,Suc(n)) = Pre(Sub(m,n))”));
+
+
 
 val Pre_O_cases = prove_store("Pre_O_case",
 e0
@@ -1084,20 +682,19 @@ e0
  “!n. Pre(n) = O <=> (n = O | n = Suc(O))”));
 
 val Pre_eq_O = Pre_O_cases
-*)
+
 
 val Le_def = qdefine_psym ("Le",[‘m:mem(N)’,‘n:mem(N)’])
                           ‘Sub(m,n) = O’
              |> gen_all |> store_as "Le_def";
 
 val Lt_def = qdefine_psym ("Lt",[‘m:mem(N)’,‘n:mem(N)’])
-                          ‘Lt(m,n) & ~(m = n)’
+                          ‘Le(m,n) & ~(m = n)’
              |> gen_all |> store_as "Lt_def";
 
 
 
-
-val SUB_EQ_00 = Le_def
+(*val SUB_EQ_00 = Le_def*)
 
 val Le_O = prove_store("Le_O",
 e0
@@ -1132,86 +729,30 @@ e0
 (form_goal
  “!n.~(Lt(n,O))”));
 
-(*
-val f = concl N_ind_P
-val f0 = “P(n) <=> Sub(Suc(m),Suc(n)) = Sub(m,n)”
-val th = (add_assum “!n:mem(N). P(n) <=> P(n)” (mk_thm(fvf f0,[],f0)))
-
-basic_fconv no_conv (rewr_fconv (spec_all th)) f
-
-
-N_ind_P |> rewr_rule[th] 
-
-
-
-
-basic_fconv no_conv (rewr_fconv (add_assum “!n:mem(N). P(n) <=> P(n)” (spec_all th)))
-
-*)
-
-
-
-(*
-local
-val l = 
- fVar_Inst 
-[("P",([("n",mem_sort N)],
- “Sub(Suc(m),Suc(n)) = Sub(m,n)”))] 
- N_ind_P 
-in
 val Sub_mono_eq = prove_store("Sub_mono_eq",
 e0
-(strip_tac >> irule l >> rw[Sub_O,Sub_Suc,Suc_def] >> 
- rpt strip_tac (* 2 *)
- >-- (pop_assum (assume_tac o GSYM) >> arw[]) >>
- rw[Pre_Suc])
-(form_goal
- “!m n. Sub(Suc(m),Suc(n)) = Sub(m,n)”));
-end
-*)
-
-
-val Sub_mono_eq = prove_store("Sub_mono_eq",
-e0
-(strip_tac >> ind_with N_ind_P >> rw[Sub_O,Sub_Suc,Suc_def] >> 
+(strip_tac >>
+ ind_with N_induct >> rw[Sub_O,Sub_Suc] >> 
  rpt strip_tac (* 2 *) >-- rw[Pre_Suc] >>
  pop_assum (assume_tac o GSYM) >> arw[])
 (form_goal
  “!m n. Sub(Suc(m),Suc(n)) = Sub(m,n)”));
 
 
-
-local
-val l = 
- fVar_Inst 
-[("P",([("c",mem_sort N)],
- “!a.Sub(Add(a,c),c) = a”))] 
- N_ind_P 
-in
 val Add_Sub = prove_store("Add_Sub",
 e0
-(rpt strip_tac >> match_mp_tac l >> rw[Suc_def,Add_Suc,Sub_mono_eq] >> 
- rw[Add_O,Sub_O])
+(ind_with N_induct >-- rw[Add_O,Sub_O] >> rpt strip_tac >>
+ arw[Add_Suc,Sub_mono_eq])
 (form_goal
  “!c a. Sub(Add(a,c),c) = a”));
-end
 
-
-
-local
-val l = 
- fVar_Inst 
-[("P",([("n",mem_sort N)],
- “Add(O,n) = n”))] 
- N_ind_P 
-in
 val Add_O2 = prove_store("Add_O2",
 e0
-(rpt strip_tac >> match_mp_tac l >> rw[Suc_def,Add_Suc,Add_O] >> 
+(ind_with N_induct >-- rw[Add_Suc,Add_O] >> 
  rpt strip_tac >> arw[])
 (form_goal
  “!n. Add(O,n) = n”));
-end
+
 
 val Sub_EQ_O = prove_store("Sub_EQ_O",
 e0
@@ -1233,8 +774,8 @@ val o_eq_l = prove_store("o_eq_l",
 e0
 (rpt strip_tac >> arw[])
 (form_goal
- “!B C g1:B~>C g2:B~>C. g1 = g2 ==>
-  !A f:A~>B. g1 o f = g2 o f”));
+ “!B C g1:B->C g2:B->C. g1 = g2 ==>
+  !A f:A->B. g1 o f = g2 o f”));
 
 val Le_cases = prove_store("Le_cases",
 e0
@@ -1243,62 +784,37 @@ e0
 (form_goal
  “!m n. Le(m,n) ==> (Lt(m,n) | m = n)”));
 
-val Le_Sub = Le_def
+val Le_Sub = Le_def;
 
 (*“!p n m.((p <= n) /\ (p <= m)) ==> (((n - p) = (m - p)) = (n = m))”*)
 
-val Suc_NONZERO = SUC_NONZERO |> rewr_rule[Suc_def]
+val Suc_NONZERO = SUC_NONZERO |> rewr_rule[GSYM Suc_def]
                               |> store_as "Suc_NONZERO";
 
-local
-val l = 
- fVar_Inst 
-[("P",([("a",mem_sort N)],
- “!b c.Le(a,b) & Le(a,c) ==>(Sub(b,a) = Sub(c,a) <=> b = c)”))] 
-N_ind_P
-val l' = 
- fVar_Inst 
-[("P",([("b",mem_sort N)],
- “!c.Le(Suc(a), b) & Le(Suc(a), c) ==>
-               (Sub(b, Suc(a)) = Sub(c, Suc(a)) <=> b = c)”))] 
-N_ind_P |> gen_all |> specl [rastt "n:mem(N)"]
-val l'' = 
- fVar_Inst 
-[("P",([("c",mem_sort N)],
- “Le(Suc(n0), App(SUC, n1)) & Le(Suc(n0), c) ==>
-               (Sub(App(SUC, n1), Suc(n0)) = Sub(c, Suc(n0)) <=>
-                 App(SUC, n1) = c)”))] 
-N_ind_P |> gen_all |> specl [rastt "n:mem(N)",rastt "n':mem(N)"]
-in
+val th = N_induct 
+
 val cancel_Sub = prove_store("cancel_Sub",
 e0
-(match_mp_tac l >> rw[Sub_O] >> rw[Suc_def] >> 
+(ind_with N_induct >> rw[Sub_O] >> 
  strip_tac >> strip_tac >> 
- match_mp_tac l' >> strip_tac (* 2 *)
- >-- (rpt strip_tac >> fs[Le_Sub,Sub_O,Suc_NONZERO]) >>
+ ind_with N_induct >> strip_tac >--
+ (rpt strip_tac >> fs[Le_Sub,Sub_O,Suc_NONZERO]) >>
  strip_tac>> strip_tac >> 
- match_mp_tac l'' >> rw[Suc_def] >> strip_tac (* 2 *)
- >-- (rpt strip_tac >> fs[Le_def,Sub_O,Suc_NONZERO]) >>
+ ind_with N_induct >> strip_tac
+ >-- fs[Le_def,Sub_O,Suc_NONZERO] >>
  rw[Sub_mono_eq,Le_def] >> rpt strip_tac >> rw[Suc_eq_eq] >>
  first_x_assum irule >> arw[Le_def])
 (form_goal
  “!a b c.Le(a,b) & Le(a,c) ==>(Sub(b,a) = Sub(c,a) <=> b = c)”));
-end
 
-local
-val l = 
- fVar_Inst 
-[("P",([("a",mem_sort N)],
- “Sub(O,a) = O”))] 
-N_ind_P
-in
+
 val Sub_of_O = prove_store("Sub_of_O",
 e0
-(match_mp_tac l >> rw[Sub_O,Sub_Suc,Suc_def] >> rpt strip_tac>>
+(ind_with N_induct >> rw[Sub_O,Sub_Suc] >> rpt strip_tac>>
  arw[Pre_O])
 (form_goal
  “!n.Sub(O,n) = O”));
-end
+
 
 val O_LESS_EQ = prove_store("O_LESS_EQ",
 e0
@@ -1334,30 +850,18 @@ e0
 (form_goal
  “!n. Le(n,O) <=> n = O”));
 
-
-local
-val l = 
- fVar_Inst 
-[("P",([("a",mem_sort N)],
- “!b. Lt(a,b) | Le(b,a)”))] 
-N_ind_P
-val l' = 
- fVar_Inst 
-[("P",([("b",mem_sort N)],
- “Lt(Suc(a),b) | Le(b,Suc(a))”))] 
-N_ind_P |> gen_all |> specl [rastt "n:mem(N)"]
-in
 val LESS_cases = prove_store("LESS_cases",
 e0
-(rpt strip_tac >> irule l >> rw[Suc_def,O_LESS_EQ] >> strip_tac 
- >-- (strip_tac >> strip_tac >> match_mp_tac l' >>
-     rw[O_LESS_EQ] >> rw[Suc_def,LESS_MONO_EQ,LESS_EQ_MONO] >> arw[]) >>
- rw[LE_O_iff] >> rw[Lt_def,O_LESS_EQ] >> strip_tac >>
- cases_on “O = b'” >> arw[])
+(ind_with N_induct >> strip_tac (* 2 *)
+ >-- (rw[LE_O_iff] >> rw[Lt_def,O_LESS_EQ] >> strip_tac >>
+     cases_on “O = b” >> arw[]) >>
+ strip_tac >> strip_tac >>
+ ind_with N_induct >> 
+ rw[O_LESS_EQ] >> rw[LESS_MONO_EQ,LESS_EQ_MONO] >> arw[])
 (form_goal
  “!a b. Lt(a,b) | Le(b,a)”));
-end
 
+ 
 val LESS_EQ_cases = prove_store("LESS_EQ_cases",
 e0
 (assume_tac LESS_cases >> fs[Lt_def] >>
@@ -1366,36 +870,21 @@ e0
 (form_goal
  “!m n. Le(m,n) | Le(n,m)”));
 
-local
-val l = 
- fVar_Inst 
-[("P",([("b",mem_sort N)],
- “!a. Add(Suc(a),b) = Suc(Add(a,b))”))] 
-N_ind_P
-in
+
 val Add_Suc1 = prove_store("Add_Suc1",
 e0
-(rpt strip_tac >> irule l >> strip_tac >> rw[Add_O] >>
- rpt strip_tac >> rw[Suc_def] >> rw[Add_Suc] >> arw[])
+(ind_with N_induct >> strip_tac >> rw[Add_O] >>
+ rpt strip_tac >> rw[Add_Suc] >> arw[])
 (form_goal
  “!b a. Add(Suc(a),b) = Suc(Add(a,b))”));
-end
 
-
-local
-val l = 
- fVar_Inst 
-[("P",([("b",mem_sort N)],
- “!a. Add(a,b) = Add(b,a)”))] 
-N_ind_P
-in
-val Add_sym = prove_store("Add_sym",
+val Add_comm = prove_store("Add_comm",
 e0
-(rpt strip_tac >> irule l >> rw[Add_O,Add_O2] >> rpt strip_tac >>
- rw[Suc_def] >> rw[Add_Suc] >> arw[] >> rw[Add_Suc1] )
+(ind_with N_induct >> rw[Add_O,Add_O2] >> rpt strip_tac >>
+ rw[Add_Suc] >> arw[] >> rw[Add_Suc1] )
 (form_goal
  “!b a. Add(a,b) = Add(b,a)”));
-end
+
 
 val Suc_Sub = prove_store("Suc_Sub",
 e0
@@ -1423,23 +912,11 @@ e0
 
 val Pre_O_cases = prove_store("Pre_O_cases",
 e0
-(rw[GSYM Pre_def]  >> assume_tac PRE_def >> strip_tac >>
- cases_on “n = O” >-- (arw[] >>
- qsuff_tac ‘ App(PRE,O) = App(PRE o El(O),dot) &  App(El(O),dot) = O’
-  >-- (rpt strip_tac >> arw[]) >> rw[El_def] >>
-  flip_tac >> irule $ iffRL App_o_l >> rw[PRE_Fun,El_Fun,El_def]) >>
- arw[] >> dimp_tac >> strip_tac (* 2 *)
- >-- (fs[O_xor_SUC] >> 
-     qpick_x_assum ‘App(SUC, pn) = n’ (assume_tac o GSYM) >>
-     fs[] >>
-     rw[GSYM Suc_def] >> rw[SUC_eq_eq] >>
-     qsuff_tac ‘App(PRE, App(SUC, pn)) = pn’ >--
-     (strip_tac >> arw[] >>
-     qpick_x_assum ‘App(PRE, App(SUC, pn)) = O’ (assume_tac o GSYM) >>
-     arw[]) >> irule $ iffLR App_o_l >> arw[App_id,SUC_Fun,PRE_Fun]) >>
- arw[] >>
- rw[GSYM Suc_def] >> irule $ iffLR App_o_l >> 
- arw[App_id,SUC_Fun,PRE_Fun])
+(strip_tac >> cases_on “n = O” (* 2 *)
+ >-- arw[Pre_O] >>
+ arw[] >> dimp_tac >> strip_tac (* 2 *) 
+ >-- (fs[O_xor_Suc,Suc_eq_eq] >> rfs[Pre_Suc]) >>
+ arw[Pre_Suc])
 (form_goal
 “!n. Pre(n) = O <=> (n = O | n = Suc(O))”));
 
@@ -1472,9 +949,7 @@ e0
 (form_goal
  “!a b. Lt(a,Suc(b)) <=> Le(a,b)”));
 
-
-
-
+(*
 fun thml_eq_pairs (th:thm,(ll,rl,asml)) = 
     if is_eq (concl th) then  
         let 
@@ -1496,6 +971,7 @@ fun EQ_fVar P thml =
             mk_thm (contl_U (List.map cont thml),asml,
                  mk_dimp (mk_fvar P ll) (mk_fvar P rl))
         end
+*)
 
 val NOT_Lt_O = prove_store("NOT_Lt_O",
 e0
@@ -1505,16 +981,6 @@ e0
  “!n. ~(Lt(n,O))”));
 
 
-
-
-
-local
-val l = 
- fVar_Inst 
-[("P",([("a",mem_sort N)],
- “!a0. Le(a0,a) ==> P(a0)”))] 
-N_ind_P
-in
 val strong_ind = prove_store("strong_ind",
 e0
 (rpt strip_tac >>
@@ -1523,7 +989,7 @@ e0
  >-- (strip_tac >> 
       pop_assum (qspecl_then [‘a:mem(N)’,‘a’] assume_tac) >>
       first_assum irule >> rw[Le_refl]) >>
- match_mp_tac l >> rw[Suc_def] >> strip_tac (* 2 *)
+ ind_with N_induct >> strip_tac (* 2 *)
  >-- (rpt strip_tac >> drule Le_O >>  
       assume_tac $ EQ_psym "P" [assume “a0 = O”] >>
       first_assum $ irule o iffRL >>
@@ -1537,16 +1003,7 @@ e0
  last_x_assum irule  >> rw[Lt_Suc_Le] >> first_x_assum accept_tac)
 (form_goal
  “(!a:mem(N).(!a0. Lt(a0,a) ==> P(a0)) ==> P(a)) ==> !a:mem(N). P(a)”));
-end
 
-
-local
-val l = 
- fVar_Inst 
-[("P",([("n",mem_sort N)],
- “!n0.Le(n0,n) ==> ~(P(n0:mem(N)))”))] 
-N_ind_P
-in
 val WOP = prove_store("WOP",
 e0
 (rpt strip_tac >> ccontra_tac >>
@@ -1566,7 +1023,7 @@ e0
  qsuff_tac ‘!n:mem(N) n0:mem(N). Le(n0,n) ==> ~P(n0)’
  >-- (strip_tac >> rpt strip_tac >> first_x_assum irule >>
      qexists_tac ‘n’ >> rw[Le_refl]) >>
- match_mp_tac l >> rpt strip_tac (* 2 *) >--
+ ind_with N_induct >> rpt strip_tac (* 2 *) >--
  (drule Le_O >>
  assume_tac $ EQ_psym "P" [assume “n0 = O”] >>
  ccontra_tac >> 
@@ -1574,7 +1031,7 @@ e0
  first_x_assum drule >>
  pop_assum strip_assume_tac >> pop_assum mp_tac >> 
  rw[Le_def,Sub_of_O]) >>
- pop_assum mp_tac >> rw[Suc_def] >> strip_tac >>
+ pop_assum mp_tac >> strip_tac >>
  drule Le_cases >> pop_assum mp_tac >> rw[Lt_Suc_Le] >> strip_tac (* 2 *)
  >-- (first_x_assum drule >> first_x_assum accept_tac) >>
  ccontra_tac >>
@@ -1589,52 +1046,22 @@ e0
  )
 (form_goal
  “!a. P(a:mem(N)) ==> ?a0. P(a0) & !a1.P(a1) ==> Le(a0,a1)”));
-end
-
-local 
-val precond = proved_th $
-e0
-(strip_tac >-- (irule o_Fun >> rw[To1_Fun,El_Fun]) >>
- irule o_Fun >> rw[ADD_Fun] >> irule Pa_Fun >>
- rw[p12_Fun] >> irule o_Fun >> rw[p1_Fun])
-(form_goal “isFun(El(O) o To1(N)) &
-      isFun(ADD o Pa(p2(N * N, N), p1(N, N) o p1(N * N, N))) ”)
-in
-val MUL_def0 = Thm1 |> allE $ rastt "N" 
-                |> allE $ rastt "N" 
-                |> allE $ rastt "El(O) o To1(N)"
-                |> allE $ rastt "ADD o Pa(p2(N * N,N),p1(N, N) o p1(N * N,N))"|> C mp precond |>  ex2fsym0 "MUL" [] |> iffRL
-                |> allE (rastt "MUL") |> rewr_rule[] 
-                |> rewr_rule[o_assoc]
-                |> store_as "MUL_def0";
-end
-
-val MUL_Fun = MUL_def0 |> conjE1 |> store_as "MUL_Fun";
-
-val MUL_def = prove_store("MUL_def",
-e0
-(rw[MUL_def0] >> irule o_eq_r >>
- irule is_To1>> irule o_Fun >> rw[To1_Fun,p1_Fun])
-(form_goal
- “MUL o Pa(p1(N, 1), El(O) o p2(N, 1)) = El(O) o To1(N * 1) &
-      ADD o Pa(p2(N * N, N), (p1(N, N) o p1(N * N, N))) o
-        Pa(id(N * N), MUL) = MUL o Pa(p1(N, N), SUC o p2(N, N))”));
 
 
-val Mul_ex = prove_store("Mul_ex",
-e0
-(rpt strip_tac >> qexists_tac ‘App(MUL,Pair(a,b))’ >> rw[])
-(form_goal “!a b.?ab. App(MUL,Pair(a,b)) = ab”));
+val MUL_def0 = Thm1 |> qspecl [‘N’,‘N’,‘El(O) o To1(N)’,
+                               ‘ADD o Pa(p2(N * N,N),p1(N, N) o p1(N * N,N))’]
+                    |> qSKOLEM "MUL" [] |> iffRL
+                    |> allE (rastt "MUL") 
+                    |> rewr_rule[o_assoc,To1_def,Pa_distr,p12_of_Pa,IdR] 
+                    |> store_as "MUL_def0";
 
-val Mul_def = Mul_ex |> spec_all |> ex2fsym0 "Mul" ["a","b"]
-                     |> gen_all |> store_as "Mul_def";
 
-val App_Pa2 = App_Pa |> sspecl [rastt "id(A)",rastt "g:B~>D"]
-                       |> rewr_rule[id_Fun,idL]
-                       |> undisch 
-                       |> gen_all |> disch_all 
-                       |> gen_all
-                       |> store_as "App_Pa2";
+
+val Mul_def = qdefine_fsym ("Mul",[‘n1:mem(N)’,‘n2:mem(N)’]) ‘App(MUL,Pair(n1,n2))’ |> gen_all |> store_as "Mul_def";
+
+val App_Pa2 = App_Pa |> qspecl [‘A’,‘A’,‘Id(A)’]
+                     |> rewr_rule[IdL] |> gen_all
+                     |> store_as "App_Pa2";
 
 val App_p1_Pair = prove_store("App_p1_Pair",
 e0
@@ -1651,114 +1078,56 @@ e0
 
 val Mul_O = prove_store("Mul_O",
 e0
-(strip_tac >> rw[GSYM Mul_def] >> 
- assume_tac MUL_def >>
+(strip_tac >> rw[Mul_def] >> 
+ assume_tac MUL_def0 >>
  qby_tac
- ‘App(MUL, Pair(n, O)) = 
-  App(MUL o Pa(p1(N, 1), El(O) o p2(N, 1)), 
-       Pair(n,dot))’ 
- >-- (flip_tac >> irule $ iffRL App_o_l >> 
-     rw[MUL_Fun] >> 
-     qsspecl_then [‘O’] assume_tac El_Fun >>
-     drule App_Pa2 >> arw[] >> rw[App_p1_Pair] >>
-     strip_tac >--
-     (irule App_input_eq >> rw[Pair_eq_eq] >>
-     irule $ iffRL App_o_l >> rw[El_Fun,p2_Fun] >>
-     rw[App_p2_Pair] >> rw[El_def]) >>
-     irule Pa_Fun >> rw[p1_Fun] >>
-     irule o_Fun >> rw[El_Fun,p2_Fun]) >>
- arw[] >> irule $ iffRL App_o_l >> 
- rw[dot_def,El_def,To1_Fun])
+ ‘App(MUL o Pa(p1(N, 1), El(O) o To1(N * 1)),Pair(n,dot)) =
+  App(El(O) o To1(N * 1),Pair(n,dot))’ 
+ >-- arw[] >>
+ pop_assum mp_tac >> 
+ rw[App_App_o,App_Pa_distr,p12_of_Pair,dot_def,El_def])
 (form_goal “!n. Mul(n,O) = O”));
 
 
 val Mul_Suc = prove_store("Mul_Suc",
 e0
-(rpt strip_tac >> rw[GSYM Mul_def,GSYM Suc_def] >>
- assume_tac MUL_def >>
+(rpt strip_tac >> rw[Mul_def,Suc_def] >>
+ assume_tac MUL_def0 >>
  qby_tac
- ‘App(MUL, Pair(n, App(SUC, n0))) = 
+ ‘App(ADD o Pa(MUL, p1(N, N)),Pair(n,n0)) = 
   App(MUL o Pa(p1(N, N), SUC o p2(N, N)),Pair(n,n0))’
- >-- (flip_tac >> irule $ iffRL App_o_l >> rw[MUL_Fun] >>
-     strip_tac >-- (irule App_input_eq >> 
-     assume_tac SUC_Fun >> drule App_Pa2 >> arw[] >>
-     rw[App_p1_Pair,Pair_eq_eq] >> irule $ iffRL App_o_l >>
-     rw[App_p2_Pair,p2_Fun,SUC_Fun]) >>
-     irule Pa_Fun >> rw[p1_Fun] >> irule o_Fun >> rw[SUC_Fun,p2_Fun]) >>
- arw[] >> 
- last_x_assum (assume_tac o GSYM) >> arw[] >>
- irule $ iffRL App_o_l >> rw[ADD_Fun] >> strip_tac 
- >-- (qspecl_then [‘N * N’,‘N’] assume_tac p2_Fun >> drule Pa_distr >>
-     qby_tac ‘isFun(p1(N,N) o p1(N * N,N))’
-     >-- (irule o_Fun >> rw[p1_Fun]) >>
-     first_x_assum drule >> 
-     qby_tac ‘isFun(Pa(id(N * N),MUL))’
-     >-- (irule Pa_Fun >> rw[id_Fun,MUL_Fun]) >>
-     first_x_assum drule >> arw[] >>
-     rw[GSYM Add_def] >> irule App_input_eq >>
-     qby_tac ‘isFun(id(N * N)) & isFun(MUL)’
-     >-- rw[id_Fun,MUL_Fun] >> drule p2_of_Pa>> arw[] >>
-     rw[o_assoc] >>
-     drule p1_of_Pa >> arw[] >> rw[idR] >> 
-     qby_tac ‘isFun(MUL) & isFun(p1(N,N))’ 
-     >-- rw[MUL_Fun,p1_Fun] >> drule App_Pa_Pair >> arw[] >>
-     rw[App_p1_Pair]) >>
- irule o_Fun >> strip_tac (* 2 *)
- >-- (irule Pa_Fun >> rw[p2_Fun] >> irule o_Fun >> rw[p1_Fun]) >>
- irule Pa_Fun >> rw[MUL_Fun,id_Fun])
+ >-- arw[] >>
+ pop_assum mp_tac >> rw[App_App_o,App_Pa_Pair,p12_of_Pair,Add_def] >>
+ strip_tac >> arw[])
 (form_goal “!n n0. Mul(n,Suc(n0)) = Add(Mul(n,n0),n)”));
 
-
-local
-val l = 
- fVar_Inst 
-[("P",([("n",mem_sort N)],
- “Mul(O,n) = O”))] 
- N_ind_P 
-in
 val Mul_LEFT_O = prove_store("Mul_LEFT_O",
 e0
-(irule l >> rw[Suc_def,Mul_O,Mul_Suc,Add_O])
+(ind_with N_induct >> rw[Mul_O,Mul_Suc,Add_O])
 (form_goal “!m. Mul(O,m) = O”));
-end
 
-local
-val l = 
- fVar_Inst 
-[("P",([("n",mem_sort N)],
- “Mul(Suc(O),n) = n”))] 
- N_ind_P 
-in
+
 val Mul_LEFT_1 = prove_store("Mul_LEFT_1",
 e0
-(irule l >> rw[Suc_def,Mul_O,Mul_Suc] >> rpt strip_tac >>
+(ind_with N_induct >> rw[Mul_O,Mul_Suc] >> rpt strip_tac >>
  arw[Add_Suc,Add_O])
 (form_goal “!m.Mul(Suc(O),m) = m”));
-end
+
 
 val Mul_RIGHT_1 = prove_store("Mul_RIGHT_1",
 e0
 (rw[Mul_Suc,Add_O2,Mul_O])
 (form_goal “!m. Mul(m,Suc(O)) = m”));
 
-val Add_sym' = GSYM Add_sym |> store_as "Add_sym'";
+val Add_comm' = GSYM Add_comm |> store_as "Add_comm'";
 
-
-
-local 
-val l =
-fVar_Inst 
-[("P",([("m",mem_sort N)],
- “!n0 p. Add(m,Add(n0,p)) = Add(Add(m,n0),p)”))] 
-N_ind_P
-in
 val Add_assoc = prove_store("Add_assoc",
 e0
-(irule l >> rw[Add_O,Suc_def,Add_Suc,Add_Suc1,Add_O2] >>
+(ind_with N_induct >> rw[Add_O,Add_Suc,Add_Suc1,Add_O2] >>
  rpt strip_tac >>arw[])
 (form_goal
  “!m n0 p. Add(m,Add(n0,p)) = Add(Add(m,n0),p)”));
-end
+
 
 val Add_eq_eq = prove_store("Add_eq_eq",
 e0
@@ -1769,143 +1138,98 @@ e0
  fs[Add_Sub])
 (form_goal
  “!m n a. Add(m,a) = Add(n,a) ==> m = n”));
+ 
 
-
-local
-val l = 
- fVar_Inst 
-[("P",([("m",mem_sort N)],
- “!a. Mul(Suc(a),m) = Add(m,Mul(a,m))”))] 
- N_ind_P 
-in
 val Mul_Suc1 = prove_store("Mul_Suc1",
 e0
-(irule l >> 
- rw[Mul_O,Add_O] >> rw[Suc_def,Mul_Suc] >> rpt strip_tac >>
+(ind_with N_induct >> 
+ rw[Mul_O,Add_O] >> rw[Mul_Suc] >> rpt strip_tac >>
  arw[] >> arw[Add_Suc] >>
- qsspecl_then [‘Suc(n)’,‘ Add(Mul(a, n), a)’] assume_tac Add_sym' >> 
+ qsspecl_then [‘Suc(n)’,‘ Add(Mul(n', n), n')’] assume_tac Add_comm' >> 
  arw[Add_Suc] >> 
- qsspecl_then [‘n’,‘Mul(a,n)’] assume_tac Add_sym' >> arw[] >>
+ qsspecl_then [‘n’,‘Mul(n',n)’] assume_tac Add_comm' >> arw[] >>
  rw[GSYM Add_assoc] >> 
- qsspecl_then [‘n’,‘a’] assume_tac Add_sym' >> arw[])
+ qsspecl_then [‘n’,‘n'’] assume_tac Add_comm' >> arw[])
 (form_goal
  “!m n. Mul(Suc(n),m) = Add(m,Mul(n,m))”));
-end
 
 
 val Mul_clauses = prove_store("Mul_clauses",
 e0
 (rw[Mul_O,Mul_Suc,Mul_Suc1,Mul_LEFT_1,Mul_RIGHT_1,Mul_LEFT_O] >>
  rpt strip_tac >--
- qsspecl_then [‘n’,‘Mul(m,n)’] accept_tac Add_sym' >> 
- qsspecl_then [‘Mul(m,n)’,‘m’] accept_tac Add_sym')
-(form_goal “!m. (Mul(O,m) = O) & (Mul(m,O) = O) & 
-                  (Mul(Suc(O),m) = m) & (Mul(m,Suc(O)) = m) &
-                  !n.(Mul(Suc(m),n) = Add(Mul(m,n),n)) &
+ qsspecl_then [‘n’,‘Mul(m,n)’] accept_tac Add_comm' >> 
+ qsspecl_then [‘Mul(m,n)’,‘m’] accept_tac Add_comm')
+(form_goal “(!m. (Mul(O,m) = O) & (Mul(m,O) = O) & 
+                  (Mul(Suc(O),m) = m) & (Mul(m,Suc(O)) = m)) &
+                !m n.(Mul(Suc(m),n) = Add(Mul(m,n),n)) &
                   (Mul(m,Suc(n)) = Add(m,Mul(m,n)))”));
 
 
-local
-val l = 
- fVar_Inst 
-[("P",([("m",mem_sort N)],
- “!n. Mul(m,n) = Mul(n,m)”))] 
- N_ind_P
-in
-val Mul_sym = prove_store("Mul_sym",
+val Mul_comm = prove_store("Mul_comm",
 e0
-(irule l >> rw[Mul_clauses,Suc_def] >>
+(ind_with N_induct >> rw[Mul_clauses,Suc_def] >>
  rpt strip_tac >> arw[] >>
- qsspecl_then [‘Mul(n',n)’,‘n'’] accept_tac Add_sym')
+ qsspecl_then [‘Mul(n',n)’,‘n'’] accept_tac Add_comm')
 (form_goal
  “!m n. Mul(m,n) = Mul(n,m)”));
-end
+
 
 val Add_clauses = prove_store("Add_clauses",
 e0
 (rw[Add_O,Add_O2,Add_Suc,Add_Suc1])
-(form_goal “(!m. Add(O,m) = m & Add(m,O) = m) & 
+(form_goal “((!m. Add(O,m) = m & Add(m,O) = m)) & 
             !m n.Add(Suc(m),n) = Suc(Add(m,n)) &
                  Add(m,Suc(n)) = Suc(Add(m,n))”));
 
 
+val Nind_tac = ind_with N_induct
 
-local
-val l = 
- fVar_Inst 
-[("P",([("p",mem_sort N)],
- “Mul(Add(a,b),p) = Add(Mul(a,p),Mul(b,p))”))] 
- N_ind_P
-in
 val RIGHT_DISTR = prove_store("RIGHT_DISTR",
 e0
-(strip_tac >> strip_tac >> irule l >> rw[Mul_clauses,Add_clauses] >>
- rw[Suc_def] >> strip_tac >> arw[] >>
+(strip_tac >> strip_tac >> Nind_tac >> rw[Mul_clauses,Add_clauses] >>
+ strip_tac >> arw[] >>
  rw[Mul_clauses,Add_clauses,GSYM Add_assoc] >> strip_tac >>
  arw[]>> 
  qsuff_tac ‘Add(n, Add(Mul(m, n'), Mul(n, n'))) = 
             Add(Mul(m, n'), Add(n, Mul(n, n')))’ 
  >-- (strip_tac >> arw[]) >>
- qsspecl_then [‘Mul(m, n')’,‘Add(n, Mul(n, n'))’] assume_tac Add_sym' >>
+ qsspecl_then [‘Mul(m, n')’,‘Add(n, Mul(n, n'))’] assume_tac Add_comm' >>
  arw[] >> 
  rw[GSYM Add_assoc] >>
- qsspecl_then [‘Mul(m, n')’,‘Mul(n, n')’] assume_tac Add_sym' >> arw[]
+ qsspecl_then [‘Mul(m, n')’,‘Mul(n, n')’] assume_tac Add_comm' >> arw[]
  )
 (form_goal “!m n p. Mul(Add(m,n),p) = Add(Mul(m,p),Mul(n,p))”));
-end
+
 
 
 val LEFT_DISTR = prove_store("LEFT_DISTR",
 e0
 (rpt strip_tac >>
- qsspecl_then [‘p’,‘Add(m,n)’] assume_tac Mul_sym >> arw[RIGHT_DISTR] >>
- qsspecl_then [‘p’,‘m’] assume_tac Mul_sym >> arw[] >>
- qsspecl_then [‘p’,‘n’] assume_tac Mul_sym >> arw[])
+ qsspecl_then [‘p’,‘Add(m,n)’] assume_tac Mul_comm >> arw[RIGHT_DISTR] >>
+ qsspecl_then [‘p’,‘m’] assume_tac Mul_comm >> arw[] >>
+ qsspecl_then [‘p’,‘n’] assume_tac Mul_comm >> arw[])
 (form_goal “!m n p. Mul(p,Add(m,n)) = Add(Mul(p,m),Mul(p,n))”));
 
 
-local
-val l = 
- fVar_Inst 
-[("P",([("a",mem_sort N)],
- “!b p. Mul(a,Mul(b,p)) = Mul(Mul(a,b),p)”))] 
- N_ind_P
-in
+
 val Mul_assoc = prove_store("Mul_assoc",
 e0
-(irule  l >>
- rw[Mul_clauses,RIGHT_DISTR,Suc_def] >> rpt strip_tac >>
+(Nind_tac>>
+ rw[Mul_clauses,RIGHT_DISTR] >> rpt strip_tac >>
  arw[] >> rw[GSYM Add_assoc])
 (form_goal “!m n p. Mul(m,Mul(n,p)) = Mul(Mul(m,n),p)”));
-end
 
 
-local 
-val l1 = 
- fVar_Inst 
-[("P",([("a",mem_sort N)],
- “!b c. Sub(a,Add(b,c)) = Sub(Sub(a,b),c)”))] 
- N_ind_P 
-val l2 = 
- fVar_Inst 
-[("P",([("b",mem_sort N)],
- “!c. Sub(a,Add(b,c)) = Sub(Sub(a,b),c)”))] 
- N_ind_P |> rewr_rule[Suc_def]
-val l3 = 
- fVar_Inst 
-[("P",([("c",mem_sort N)],
- “Sub(a,Add(b,c)) = Sub(Sub(a,b),c)”))] 
- N_ind_P |> rewr_rule[Suc_def]
-in
 val Sub_Add = prove_store("SUB_Add",
 e0
-(strip_tac >> match_mp_tac l1 >> rw[Sub_of_O] >> strip_tac >>
- strip_tac >> rw[Suc_def] >> strip_tac >> match_mp_tac l2 >>
+(Nind_tac >> rw[Sub_of_O] >> strip_tac >>
+ strip_tac >> Nind_tac >>
  rw[Add_O2,Sub_O] >> strip_tac >> strip_tac >>
- match_mp_tac l3 >> rw[Sub_O,Add_O] >> rpt strip_tac >>
+ Nind_tac  >> rw[Sub_O,Add_O] >> rpt strip_tac >>
  rw[Add_Suc1] >> rw[Sub_mono_eq] >> arw[])
 (form_goal “!a b c. Sub(a,Add(b,c)) = Sub(Sub(a,b),c)”));
-end
+
 
 val Le_O_iff = prove_store("Le_O_iff",
 e0
@@ -1922,16 +1246,9 @@ e0
  arw[])
 (form_goal “!a b. Le(a,Suc(b)) ==> (Le(a,b) | a = Suc(b))”));
 
-local
-val l = 
- fVar_Inst 
-[("P",([("a",mem_sort N)],
- “!b.  Le(b,a) ==> ?p. Add(p,b) = a”))] 
- N_ind_P 
-in
 val Le_Add_ex = prove_store("Le_Add_ex",
 e0
-(strip_tac >> match_mp_tac l >> rw[Suc_def,Le_O_iff] >>
+(Nind_tac >> rw[Le_O_iff] >>
  rpt strip_tac (* 2 *)
  >-- (arw[] >> qexists_tac ‘O’ >> rw[Add_O]) >>
  rpt strip_tac >> drule Le_Suc >> 
@@ -1942,25 +1259,23 @@ e0
  arw[] >> qexists_tac ‘O’ >> rw[Add_O2])
 (form_goal
  “!m n. Le(n,m) ==> ?p. Add(p,n) = m”));
-end
+
+
 
 
 val LE_def = 
-fVar_Inst 
-[("P",([("m",mem_sort N),("n",mem_sort N)],
- “Sub(m,n) = O”))] 
-(AX1 |> qspecl [‘N’, ‘N’] |> uex_expand)
-|> ex2fsym0 "LE" [] |> conjE1
+AX1 |> qspecl [‘N’, ‘N’] |> uex2ex_rule
+|> fVar_sInst_th “P(m:mem(N),n:mem(N))” “Sub(m,n) = O”
+|> qSKOLEM "LE" []
 |> store_as "LE_def";
 
 
 val LT_def = 
-fVar_Inst 
-[("P",([("m",mem_sort N),("n",mem_sort N)],
- “Holds(LE,m,n) & ~(m = n)”))] 
-(AX1 |> qspecl [‘N’, ‘N’] |> uex_expand)
-|> ex2fsym0 "LT" [] |> conjE1
+AX1 |> qspecl [‘N’, ‘N’] |> uex2ex_rule
+|> fVar_sInst_th “P(m:mem(N),n:mem(N))” “Holds(LE,m,n) & ~(m = n)”
+|> qSKOLEM "LT" []
 |> store_as "LT_def";
+
 
 val LE_Le = prove_store("LE_Le",
 e0
@@ -1982,40 +1297,25 @@ e0
 (rw[Trans_def,LE_Le] >> rpt strip_tac >>
  rw[Le_def] >> drule Le_Add_ex >>
  pop_assum (strip_assume_tac o GSYM) >> arw[] >>
- qsspecl_then [‘a2’,‘p’] assume_tac Add_sym >> 
+ qsspecl_then [‘a2’,‘p’] assume_tac Add_comm >> 
  once_arw[] >> rw[Sub_Add] >> fs[Le_def] >>
  rw[Sub_of_O])
 (form_goal “Trans(LE)”));
 
 
-local
-val l = 
- fVar_Inst 
-[("P",([("p",mem_sort N)],
- “Lt(a,b) <=> Lt(Add(a,p),Add(b,p))”))] 
- N_ind_P 
-in
 val LESS_MONO_ADD = prove_store("LESS_MONO_ADD",
 e0
-(strip_tac >> strip_tac >> match_mp_tac l >>
- rw[Suc_def] >> rw[Add_O,Add_Suc,LESS_MONO_EQ])
+(strip_tac >> strip_tac >> Nind_tac >>
+ rw[Add_O,Add_Suc,LESS_MONO_EQ])
 (form_goal “!m n p. Lt(m,n) <=> Lt(Add(m,p),Add(n,p))”));
-end
 
-local
-val l = 
- fVar_Inst 
-[("P",([("p",mem_sort N)],
- “(Add(a,p) = Add(b,p)) <=> a = b”))] 
- N_ind_P 
-in
 val EQ_MONO_ADD_EQ = prove_store("EQ_MONO_ADD_EQ",
 e0
-(strip_tac >> strip_tac >> match_mp_tac l >>
- rw[Add_O,Suc_def,Add_Suc] >> rpt strip_tac >>
+(strip_tac >> strip_tac >> Nind_tac >> 
+ rw[Add_O,Add_Suc] >> rpt strip_tac >> 
  arw[Suc_eq_eq])
 (form_goal “!m n p.(Add(m,p) = Add(n,p)) <=> m = n”));
-end
+
 
 val LESS_MONO_ADD_EQ = GSYM LESS_MONO_ADD
                             |> store_as 
@@ -2044,11 +1344,10 @@ val Le_Add = prove_store("Le_Add",
 e0
 (rpt strip_tac >> irule Le_trans >>
  qexists_tac ‘Add(a,d)’ >> arw[LESS_EQ_MONO_ADD_EQ] >>
- qsspecl_then [‘b’,‘a’] assume_tac Add_sym >>
+ qsspecl_then [‘b’,‘a’] assume_tac Add_comm >>
  arw[] >>
- qsspecl_then [‘d’,‘a’] assume_tac Add_sym >>
- arw[] >> arw[LESS_EQ_MONO_ADD_EQ]
-(*need sub of add*))
+ qsspecl_then [‘d’,‘a’] assume_tac Add_comm >>
+ arw[] >> arw[LESS_EQ_MONO_ADD_EQ])
 (form_goal
  “!a b c d. Le(a,c) & Le(b,d) ==> 
    Le(Add(a,b),Add(c,d))”));
@@ -2056,18 +1355,18 @@ e0
 
 
 
+
 val _ = new_pred "Asym" [("R",rel_sort (mk_set "A") (mk_set "A"))]
 
-val Asym_def = store_ax("Asym_def",“!A R:A~>A. Asym(R) <=> 
-!a b. Holds(R,a,b) & Holds(R,b,a) ==> a = b”)
+val Asym_def = qdefine_psym("Asym",[‘R:A~>A’]) ‘!a b. Holds(R,a,b) & Holds(R,b,a) ==> a = b’ |> gen_all |> store_as "Asym_def";
 
 
 
 local
 val l = 
- fVar_Inst 
-[("P",([("a",mem_sort N)],
- “a = Suc(a)”))] 
+ fVar_Inst_th
+("P",([("a",mem_sort (rastt "N"))],
+ “a = Suc(a)”))
  WOP 
 in
 val Suc_NEQ = prove_store("Add_Suc_NEQ",
@@ -2090,23 +1389,15 @@ e0
 (form_goal “!a. Lt(a,Suc(a))”));
 
 
-
-local
-val l = 
- fVar_Inst 
-[("P",([("b",mem_sort N)],
- “Lt(a,Add(a,Suc(b)))”))] 
- N_ind_P 
-in
 val Add_Suc_Lt = prove_store("Add_Suc_NEQ",
 e0
-(strip_tac >> match_mp_tac l >> rw[Suc_def] >> strip_tac 
+(strip_tac >> Nind_tac >> strip_tac    
  >-- (rw[Lt_def,Le_def,Add_Suc,Add_O,Sub_Suc,Pre_O,O_xor_Suc,
         Suc_NEQ,Pre_O,Sub_EQ_O]) >>
  rpt strip_tac >> rw[Add_Suc] >> rw[Lt_Suc_Le] >>
  rw[GSYM Add_Suc] >> fs[Lt_def])
 (form_goal “!a b. Lt(a,Add(a,Suc(b)))”));
-end
+ 
 
 
 
@@ -2123,8 +1414,8 @@ e0
   qby_tac ‘~(p' = O)’ >-- 
   (ccontra_tac >> fs[Add_O2]) >>
   fs[O_xor_Suc] >> strip_tac
- >-- (qexists_tac ‘pn'’ >> once_rw[Add_sym] >> fs[]) >>
- qexists_tac ‘pn’ >> once_rw[Add_sym] >> fs[]) >>
+ >-- (qexists_tac ‘pn'’ >> once_rw[Add_comm] >> fs[]) >>
+ qexists_tac ‘pn’ >> once_rw[Add_comm] >> fs[]) >>
  pop_assum (strip_assume_tac o GSYM) >>
  fs[] >> rw[GSYM Add_assoc] >> once_rw[Add_Suc] >>
  assume_tac Add_Suc_Lt >> fs[Lt_def])
@@ -2142,7 +1433,7 @@ e0
  qexists_tac ‘b’ >> arw[]) >> fs[Lt_def])
 (form_goal “Asym(LE)”));
 
-val Le_asym = LE_Asym |> rewr_rule[LE_Le,Asym_def]
+val Le_Asym = LE_Asym |> rewr_rule[LE_Le,Asym_def]
                       |> store_as "Le_Asym";
 
 
@@ -2151,24 +1442,21 @@ val LESS_EQ_LESS_EQ_MONO = prove_store("LESS_EQ_LESS_EQ_MONO",
 e0
 (rpt strip_tac >> irule Le_trans >>
  qexists_tac ‘Add(m,q)’ >> arw[LESS_EQ_MONO_ADD_EQ] >>
- once_rw[Add_sym] >> arw[LESS_EQ_MONO_ADD_EQ])
+ once_rw[Add_comm] >> arw[LESS_EQ_MONO_ADD_EQ])
 (form_goal “!m n p q. (Le(m,p) & Le(n,q)) ==> Le(Add(m,n),Add(p,q))”));
 
-local
-val l = 
- fVar_Inst 
-[("P",([("p",mem_sort N)],
- “Le(a,b) ==> Le(Mul(a,p),Mul(b,p))”))] 
- N_ind_P 
-in
+
+
+
 val Le_MONO_Mul = prove_store("Le_MONO_Mul",
 e0
-(strip_tac >> strip_tac >> match_mp_tac l >> 
- rw[Mul_O,Le_refl,Suc_def] >> strip_tac >> arw[] >>
+(strip_tac >> strip_tac >> Nind_tac >>
+ rw[Mul_O,Le_refl] >> strip_tac >> arw[] >>
  rw[Mul_Suc] >> rpt strip_tac >>
  first_x_assum drule >> irule LESS_EQ_LESS_EQ_MONO >> arw[])
 (form_goal “!m n p. Le(m,n) ==> Le(Mul(m,p),Mul(n,p))”));
-end
+
+
 
 val Le_MONO_Mul' = Le_MONO_Mul |> strip_all_and_imp
                                |> gen_all
@@ -2181,7 +1469,7 @@ e0
 (rpt strip_tac >> 
  irule Le_trans >> qexists_tac ‘Mul(m,j)’ >> 
  rev_drule Le_MONO_Mul' >> arw[] >>
- drule Le_MONO_Mul' >> once_rw[Mul_sym] >> arw[])
+ drule Le_MONO_Mul' >> once_rw[Mul_comm] >> arw[])
 (form_goal “!m n i j. Le(m,i) & Le(n,j) ==> Le(Mul(m,n),Mul(i,j))”));
 
 
@@ -2192,28 +1480,15 @@ e0
 (rw[Le_def,Sub_of_O])
 (form_goal “!x. Le(O,x)”));
 
-local
-val l = 
- fVar_Inst 
-[("P",([("a",mem_sort N)],
- “!b.Le(b,a) ==> Sub(Suc(a),b) = Suc(Sub(a,b))”))] 
- N_ind_P 
-val l' = 
- fVar_Inst 
-[("P",([("b'",mem_sort N)],
- “Le(b', Suc(r)) ==>
-               Sub(Suc(Suc(r)), b') = Suc(Sub(Suc(r), b'))”))] 
- N_ind_P 
-in
 val Sub_Suc1 = prove_store("Sub_Suc1",
 e0
-(match_mp_tac l >>
+(Nind_tac >> 
  rw[Le_O_iff,Sub_of_O] >> strip_tac (* 2 *)
  >-- (rpt strip_tac >> arw[Sub_O]) >>
- strip_tac >> strip_tac >> rw[Suc_def] >>
- match_mp_tac l' >>
+ strip_tac >> strip_tac >> 
+ Nind_tac >> 
  arw[] >> rw[Le_O,Sub_O] >> strip_tac >>
- rw[Suc_def] >> arw[] >>
+ arw[] >>
  rw[Le_MONO] >> rw[Sub_Suc] >> rpt strip_tac >>
  qby_tac ‘Le(n',Suc(n))’ 
  >-- (irule Le_trans >> qexists_tac ‘n’ >> arw[] >>
@@ -2222,29 +1497,17 @@ e0
  last_x_assum drule >> arw[] >> rw[Pre_Suc])
 (form_goal
  “!a b. Le(b,a) ==> Sub(Suc(a),b) = Suc(Sub(a,b))”));
-end
 
 
-local
-val l = 
- fVar_Inst 
-[("P",([("a",mem_sort N)],
- “!b. Le(b,a) ==> Add(Sub(a,b),b) = a”))] 
- N_ind_P 
-val l' = 
- fVar_Inst 
-[("P",([("b",mem_sort N)],
- “Le(b, Suc(n)) ==> Add(Sub(Suc(n), b), b) = Suc(n)”))] 
- N_ind_P 
-in
+
 val SUB_ADD = prove_store("SUB_ADD",
 e0
-(match_mp_tac l >> 
+(Nind_tac >> 
  rw[Sub_of_O,Add_O2,Le_O_iff] >> strip_tac >>
- strip_tac >> rw[Suc_def] >>
- match_mp_tac l' >>
+ strip_tac >>
+ Nind_tac >> 
  rw[Sub_O,Add_Suc1,Add_O] >> strip_tac >> arw[] >>
- rw[Suc_def] >> rw[Sub_mono_eq] >> rw[Add_Suc] >> 
+ rw[Sub_mono_eq] >> rw[Add_Suc] >> 
  rw[Suc_eq_eq] >> rw[Le_MONO] >> 
  rpt strip_tac >> 
  qby_tac ‘Le(n',Suc(n))’ 
@@ -2253,35 +1516,22 @@ e0
  first_x_assum drule >> rev_drule Sub_Suc1 >> fs[] >> 
  first_x_assum irule >> arw[])
 (form_goal “!m n. Le(n,m) ==> Add(Sub(m,n),n) = m”));
-end
 
 
 
-local
-val l = 
- fVar_Inst 
-[("P",([("n",mem_sort N)],
- “!p. Le(n,p) ==> (Add(m,n) = p <=> m = Sub(p,n))”))] 
- N_ind_P 
-val l' = 
- fVar_Inst 
-[("P",([("p'",mem_sort N)],
- “Le(Suc(n'), p') ==>
-  (Add(m, Suc(n')) = p' <=> m = Sub(p', Suc(n')))”))] 
- N_ind_P 
-in
+
 val ADD_EQ_SUB = prove_store("ADD_EQ_SUB",
 e0
-(strip_tac >> match_mp_tac l >> 
- rw[Le_O_iff,Add_O,Sub_O,Suc_def] >> strip_tac >> strip_tac >>
- match_mp_tac l' >> rw[Suc_def] >> 
+(strip_tac >> Nind_tac >>
+ rw[Le_O_iff,Add_O,Sub_O] >> strip_tac >> strip_tac >>
+ Nind_tac >>
  rw[Le_def,Sub_O,Suc_NONZERO] >> strip_tac >> arw[] >>
  rw[Add_Suc,Suc_eq_eq,Le_MONO,Sub_mono_eq] >>rpt strip_tac >>
  fs[GSYM Le_def] >>
  first_x_assum drule >> arw[])
 (form_goal
  “!m n p. Le(n,p) ==> (Add(m,n) = p <=> m = Sub(p,n))”));
-end
+
 
 val NOT_SUC_LESS_EQ_O = prove_store("NOT_SUC_LESS_EQ_O",
 e0
@@ -2297,35 +1547,23 @@ e0
 
 val Lt_MONO = LESS_MONO_EQ |> store_as "Lt_MONO"; 
 
-local
-val l = 
- fVar_Inst 
-[("P",([("a",mem_sort N)],
- “!b.~Lt(a, b) <=> Le(b, a)”))] 
- N_ind_P 
-val l' = 
- fVar_Inst 
-[("P",([("b",mem_sort N)],
- “~Lt(Suc(n'), b) <=> Le(b, Suc(n'))”))] 
- N_ind_P 
-in
+
 val NOT_LESS = prove_store("NOT_LESS",
 e0
-(match_mp_tac l >>
- rw[Suc_def] >> rw[Le_O_iff] >> strip_tac (* 2 *)
+(Nind_tac >> rw[Le_O_iff] >> strip_tac (* 2 *)
  >-- (strip_tac >> dimp_tac >> strip_tac >>
-     ccontra_tac >> fs[O_xor_SUC,Suc_def] >> fs[Lt_def,GSYM Suc_NONZERO]>>
+     ccontra_tac >> fs[O_xor_Suc] >> fs[Lt_def,GSYM Suc_NONZERO]>>
      fs[Le_def,Sub_Suc,Sub_of_O,Pre_O] >> rfs[] >>
      last_x_assum (assume_tac o GSYM) >> fs[Suc_NONZERO]) >>
  strip_tac >> strip_tac >>
- match_mp_tac l' >> rw[NOT_SUC_LT_O,Le_O'] >>
- rw[Suc_def] >> strip_tac >> arw[] >>
+ Nind_tac >> rw[NOT_SUC_LT_O,Le_O'] >>
+ strip_tac >> arw[] >>
  rw[Le_MONO,Lt_MONO] >> arw[])
 (form_goal “!m n. ~(Lt(m,n)) <=> Le(n,m)”));
-end
 
 
 
+ 
 val RIGHT_SUB_DISTR = prove_store("RIGHT_SUB_DISTR",
 e0
 (rpt strip_tac >>
@@ -2342,7 +1580,7 @@ e0
 
 val LEFT_SUB_DISTR = prove_store("LEFT_SUB_DISTR",
 e0
-(rpt strip_tac >> once_rw[Mul_sym] >>
+(rpt strip_tac >> once_rw[Mul_comm] >>
  rw[RIGHT_SUB_DISTR])
 (form_goal “!m n p. Mul(p,Sub(m,n)) = Sub(Mul(p,m),Mul(p,n))”));
 
@@ -2394,3 +1632,6 @@ val PRE_def0 = Nind_def |> specl [rastt "N * N"]
                         |> specl [rastt "SUC"]
                         |> C mp SUC_Fun 
 *)                        
+
+
+
