ztest.sml
@@ -1,3 +1,119 @@
+val ZR_def = 
+AX1 |> qspecl [‘N * N’,‘N * N’] |> uex2ex_rule
+    |> fVar_sInst_th “P(mn:mem(N * N),m'n':mem(N * N))”
+       “Add(Fst(mn:mem(N * N)),Snd(m'n':mem(N * N))) = 
+        Add(Fst(m'n'),Snd(mn))”
+    |> qSKOLEM "ZR" [] |> store_as "ZR_def";
+
+
+val ZR_Refl = prove_store("ZR_Refl",
+e0
+(rw[Refl_def,ZR_def])
+(form_goal
+ “Refl(ZR)”));
+
+
+
+val ZR_ER = prove_store("ZR_ER",
+e0
+(cheat)
+(form_goal “ER(ZR)”));
+
+
+val Sg_ex = prove_store("Sg_ex",
+e0
+(cheat)
+(form_goal “!A. ?Sg:A-> Pow(A). 
+ !a a'.IN(a',App(Sg,a)) <=> a' = a”));
+
+val Sg_def = Sg_ex |> spec_all |> qSKOLEM"Sg" [‘A’] 
+                   |> gen_all
+                   |> store_as "Sg_def";
+
+
+val Sing_ex = prove_store("Sing_ex",
+e0
+(cheat)
+(form_goal
+ “!A a:mem(A).?sa. sa = App(Sg(A),a)”));
+
+val Sing_def = qdefine_fsym ("Sing",[‘a:mem(A)’])
+                            ‘App(Sg(A),a:mem(A))’
+                            |> gen_all |> store_as "Sing_def";
+
+
+val Ri_ex = prove_store("Ri_ex",
+e0
+(cheat)
+(form_goal “!A B r:A~>B. ?Ri:Pow(A) -> Pow(B).
+ !s b. IN(b,App(Ri,s)) <=> ?a. IN(a,s) & Holds(r,a,b)”));
+
+val Ri_def = Ri_ex |> spec_all |> qSKOLEM "Ri" [‘r’] 
+                   |> gen_all |> store_as "Ri_def";
+
+(*Relational singleton image*)
+val Rsi_def = qdefine_fsym ("Rsi",[‘r:A~>B’])
+                            ‘Ri(r:A~>B) o Sg(A)’
+                            |> gen_all |> store_as "Rsi_def";
+
+
+val rsi_def = qdefine_fsym ("rsi",[‘r:A~>B’,‘a:mem(A)’])
+                            ‘App(Rsi(r),a)’
+                            |> gen_all |> store_as "rsi_def";
+
+
+
+val rsi_eq_ER = prove_store("rsi_eq_ER",
+e0
+(cheat)
+(form_goal “!A r:A~>A.ER(r) ==> 
+ !a1 a2. rsi(r,a1) = rsi(r,a2) <=> Holds(r,a1,a2)”));
+
+
+val Z_def = Thm_2_4 |> qspecl [‘Pow(N * N)’]
+                    |> fVar_sInst_th “P(s:mem(Pow(N * N)))”
+                    “?n. s = rsi(ZR,n)”
+                    |> qSKOLEM "Z" []
+                    |> qSKOLEM "iZ" []
+                    |> store_as "Z_def";
+
+val iZ_Inj = Z_def |> conjE1 |> store_as "iZ_Inj"
+                   |> store_as "iZ_Inj";
+
+
+(*as in iN_eq_eq*)
+val iZ_eq_eq = iZ_Inj |> rewr_rule[Inj_def]
+     
+
+(* (?(n : mem(N * N)). a# = rsi(ZR, n#)) <=>
+ ?n1 n2. ... such a conv, to corresponds to L's lambda ver *)
+
+(*compare to iN_inNs*)
+val iZ_rsi = prove_store("iZ_rsi",
+e0
+(strip_tac >> strip_assume_tac Z_def >>
+ first_x_assum (qspecl_then [‘App(iZ,z)’] assume_tac) >>
+ (*stupid step, ?(b : mem(Z)). App(iZ, z) = App(iZ, b#)*)
+ qby_tac ‘?b. App(iZ,z) = App(iZ,b)’ 
+ >-- (qexists_tac ‘z’ >> rw[]) >>
+ first_x_assum (drule o iffRL) >>
+ pop_assum strip_assume_tac >>
+ qsspecl_then [‘n’] strip_assume_tac Pair_has_comp >>
+ fs[] >> qexistsl_tac [‘a’,‘b’] >> arw[]
+ )
+(form_goal 
+ “!z:mem(Z).?m n. App(iZ,z) = rsi(ZR,Pair(m,n))”));
+
+val rsi_iZ = prove_store("rsi_iZ",
+e0
+(rpt strip_tac >> strip_assume_tac Z_def >>
+ first_x_assum
+ (qspecl_then [‘rsi(ZR,Pair(m,n))’] assume_tac) >>
+ first_x_assum $ irule o iffLR >>
+ qexists_tac ‘Pair(m,n)’ >> rw[])
+(form_goal 
+ “!m n. ?z. rsi(ZR,Pair(m,n)) = App(iZ,z)”));
+
 
 val resp_def = 
  qdefine_psym("resp",[‘f:A->B’,‘r1:A~>A’,‘r2:B~>B’])
@@ -22,18 +138,6 @@ val rext_def = rext_ex |> spec_all
                        [‘f’,‘r1’,‘r2’]
                        |> gen_all |> store_as "rext_def";
 
-val main = prove_store("main",
-e0
-cheat
-(form_goal
-“!A B f:A->B r1:A~>A r2:B~>B
- Q1 Q2 i1:Q1->Pow(A) i2:Q2->Pow(B). 
- ER(r1) & ER(r2) & resp(f,r1,r2) &
- (!sa. (?q1. sa = App(i1,q1)) <=> (?a. sa = rsi(r1,a))) & 
- (!sb. (?q2. sb = App(i2,q2)) <=> (?b. sb = rsi(r2,b))) ==>
- ?qf: Q1-> Q2.
- !q1:mem(Q1). Holds(rext(f,r1,r2),App(i1,q1),App(i2 o qf,q1)) ”));
-
 (* product rel *)
 val prrel_ex = prove_store("prrel_ex",
 e0
@@ -47,6 +151,55 @@ val prrel_def = prrel_ex |> spec_all |> qSKOLEM "prrel"
 
 
 
+
+val main = prove_store("main",
+e0
+(rpt strip_tac >> assume_tac 
+ (P2fun' |> qspecl [‘Q1’,‘Q2’] 
+        |> fVar_sInst_th “P(q1:mem(Q1),q2:mem(Q2))”
+           “Holds(rext(f:A->B, r1, r2), 
+                      App(i1:Q1->Pow(A), q1), 
+                      App(i2:Q2->Pow(B), q2))”) >>
+ rw[App_App_o] >> first_x_assum irule >>
+ strip_tac >> 
+ qby_tac
+ ‘!sb.(?!q2. sb = App(i2,q2)) <=> 
+       ?b. sb = rsi(r2,b)’ >-- cheat (* easy by injection*)>>
+ fs[resp_def] >>
+ first_x_assum (qspecl_then [‘App(i1,x)’] assume_tac) >>
+ qby_tac ‘?a. App(i1,x) = rsi(r1,a)’ >-- cheat >>
+ (*should be auto*)
+ pop_assum strip_assume_tac >>
+ first_x_assum (qspecl_then [‘App(Rsi(r2) o f,a)’] 
+ assume_tac) >> fs[GSYM rsi_def,App_App_o] >>
+ qby_tac
+ ‘?!q2:mem(Q2). rsi(r2, App(f, a)) = App(i2, q2)’
+ >-- cheat >>
+ qsuff_tac ‘!q2:mem(Q2). 
+  rsi(r2, App(f, a)) = App(i2, q2) <=> 
+  Holds(rext(f, r1, r2), rsi(r1, a), App(i2, q2))’
+ >-- cheat >>
+ rw[rext_def] >> strip_tac >> dimp_tac >> strip_tac (* 2 *)
+ >-- (qexistsl_tac [‘a’,‘App(f,a)’] >> arw[]) >>
+ qsuff_tac ‘?b. App(i2, q2) = rsi(r2, b) & 
+ Holds(r2,b,App(f, a))’ >-- 
+ (strip_tac >> 
+ qpick_x_assum ‘App(i2, q2) = rsi(r2, b')’
+ (assume_tac o GSYM) >> arw[] >>
+ qby_tac ‘Holds(r2,b,b')’ >-- cheat (*by assum*) >>
+ cheat) >>
+ qexists_tac ‘b’ >> arw[] >> pop_assum (assume_tac o GSYM) >>
+ arw[] >> first_x_assum irule >> cheat
+ (*final cheat by assum rsi(r1, a) = rsi(r1, a') *))
+(form_goal
+“!A B f:A->B r1:A~>A r2:B~>B
+ Q1 Q2 i1:Q1->Pow(A) i2:Q2->Pow(B). 
+ ER(r1) & ER(r2) & resp(f,r1,r2) & Inj(i1) & Inj(i2) &
+ (!sa. (?q1. sa = App(i1,q1)) <=> (?a. sa = rsi(r1,a))) & 
+ (!sb. (?q2. sb = App(i2,q2)) <=> (?b. sb = rsi(r2,b))) ==>
+ ?qf: Q1-> Q2.
+ !q1:mem(Q1). Holds(rext(f,r1,r2),App(i1,q1),App(i2 o qf,q1)) ”));
+
 val main = prove_store("main",
 e0
 cheat
@@ -58,6 +211,8 @@ cheat
  (!sb. (?q2. sb = App(i2,q2)) <=> (?b. sb = rsi(r2,b))) ==>
  ?qf: Q1-> Q2.
  !q1:mem(Q1). Holds(rext(f,r1,r2),App(i1,q1),App(i2 o qf,q1)) ”));
+
+
 
 (*
 
@@ -80,6 +235,31 @@ val ipow2_def = ipow2_ex |> spec_all
                          |> qSKOLEM "ipow2" [‘i1’,‘i2’]
                          |> gen_all
 
+
+
+val addf0_def = proved_th $
+e0
+cheat
+(form_goal “?f:(N * N) * N * N -> N * N. 
+ !x y u v. App(f,Pair(Pair(x,y),Pair(u,v))) = 
+ Pair(Add(x,u),Add(y,v))”)
+|> qSKOLEM "addf0" []
+|> store_as "addf0_def";
+
+
+val negf0_def = fun_tm_compr (dest_var $ rastt "mn:mem(N * N)")
+                         (rastt "Pair(Snd(mn:mem(N * N)),Fst(mn))") |> qSKOLEM "negf0" []
+      |> store_as "negf0_def";
+
+
+val negf0_def1 = 
+    negf0_def |> qspecl [‘Pair(m:mem(N),n:mem(N))’]
+              |> rewr_rule[Pair_def']
+              |> gen_all |> store_as "negf0_def1";
+
+
+
+val main_addz = 
 main |> qspecl [‘(N * N) * (N * N)’,‘N * N’,
                 ‘addf0’,
                 ‘prrel(ZR,ZR)’,‘ZR’,
@@ -89,16 +269,164 @@ main |> qspecl [‘(N * N) * (N * N)’,‘N * N’,
 
 
 
+val addz_ex = prove_store("addz_ex",
+e0
+(cheat)
+(form_goal
+ “?qf: Z* Z ->Z.
+     !q1 : mem(Z * Z).
+ Holds(rext(addf0, prrel(ZR, ZR), ZR), App(ipow2(iZ, iZ), q1),App(iZ o qf, q1))”));
+
+val addz_def = addz_ex |> qSKOLEM "addz" []
 
 
-“Rsi(prrel(ZR,ZR)) = a”
-(*lift_fun_rel*)
-val Lfr_def =
-    AX1 |> qspecl [‘Y’,‘Y’] |> uex2ex_rule 
-        |> fVar_sInst_th “P(y1:mem(Y),y2:mem(Y))”
-           “?x1 x2. y1 = App(enc1:X->Y,x1) &
-                    y2 = App(enc2,x2) & App(f,x1) = x2”
-        |> qSKOLEM "Lfr" [‘f’,‘enc’]
-        |> gen_all
-        |> store_as "Lfr_def";
+val Addz_def = proved_th $
+e0
+cheat
+(form_goal “!z1 z2.?z. z = App(addz,Pair(z1,z2))”)
+|> spec_all |> qSKOLEM "Addz" [‘z1’,‘z2’]
+|> gen_all
 
+
+val addz_property = 
+    addz_def |> rewr_rule[rext_def]
+             |> qspecl [‘Pair(z1:mem(Z),z2:mem(Z))’]
+             |> rewr_rule[App_App_o,GSYM Addz_def]
+
+val addz_prop1 = prove_store("addz_prop1",
+e0
+cheat
+(form_goal
+ “?x y u v a b.
+        App(ipow2(iZ, iZ), Pair(z1, z2)) = 
+        rsi(prrel(ZR, ZR), Pair(Pair(x,y),Pair(u,v))) &
+        App(iZ, Addz(z1, z2)) = rsi(ZR, Pair(a,b)) & 
+        App(addf0, Pair(Pair(x,y),Pair(u,v))) = Pair(a,b)”));
+
+
+val addz_prop2 = prove_store("addz_prop2",
+e0
+cheat
+(form_goal
+ “?x y u v.
+        App(ipow2(iZ, iZ), Pair(z1, z2)) = 
+        rsi(prrel(ZR, ZR), Pair(Pair(x,y),Pair(u,v))) &
+        App(iZ, Addz(z1, z2)) = rsi(ZR, Pair(Add(x,u),Add(y,v)))”));
+
+
+val addz_prop3 = prove_store("addz_prop3",
+e0
+cheat
+(form_goal
+ “?x y u v.
+   (!a b c d.
+            IN(Pair(Pair(a,b),Pair(c,d)), App(ipow2(iZ, iZ), Pair(z1, z2))) <=>
+            IN(Pair(Pair(a,b),Pair(c,d)), rsi(prrel(ZR, ZR), Pair(Pair(x, y), Pair(u, v)))))  &
+        App(iZ, Addz(z1, z2)) = rsi(ZR, Pair(Add(x,u),Add(y,v)))”));
+
+
+val addz_prop4 = addz_prop3 |> rewr_rule[ipow2_def]
+
+
+
+val addz_prop5 = prove_store("addz_prop5",
+e0
+cheat
+(form_goal
+ “!z1 z2.?x y u v.
+   (!a b c d.
+     IN(Pair(a, b), App(iZ, z1)) & 
+     IN(Pair(c, d), App(iZ, z2)) <=>
+     IN(Pair(a, b), rsi(ZR,Pair(x,y))) & 
+     IN(Pair(c, d), rsi(ZR,Pair(u,v))
+   ))  &
+        App(iZ, Addz(z1, z2)) = rsi(ZR, Pair(Add(x,u),Add(y,v)))”));
+
+
+val addz_prop6 = prove_store("addz_prop6",
+e0
+cheat
+(form_goal
+ “!z1 z2.?x y u v.
+   App(iZ,z1) = rsi(ZR,Pair(x,y)) & 
+   App(iZ,z2) = rsi(ZR,Pair(u,v)) &
+   App(iZ, Addz(z1, z2)) = rsi(ZR, Pair(Add(x,u),Add(y,v)))”));
+
+(*claim: 7 can be automated from 6*)
+val addz_prop7 = prove_store("addz_prop7",
+e0
+cheat
+(form_goal
+ “!z1 z2 x y u v.
+   App(iZ,z1) = rsi(ZR,Pair(x,y)) & 
+   App(iZ,z2) = rsi(ZR,Pair(u,v)) ==> 
+   App(iZ, Addz(z1, z2)) = rsi(ZR, Pair(Add(x,u),Add(y,v)))”));
+
+
+val addf0_sym_cong = prove_store("addf0_sym_cong",
+e0
+cheat
+(form_goal “!ab cd. Holds(ZR,App(addf0,Pair(ab,cd)),
+                     App(addf0,Pair(cd,ab)))”));
+
+val rsi_eq_ZR = rsi_eq_ER |> qsspecl [‘ZR’] 
+                          |> C mp ZR_ER
+
+
+
+val eq_ZR = prove_store("eq_ZR",
+e0
+(cheat)
+(form_goal
+ “!a b. a = b ==> Holds(ZR,a,b)”));
+
+(*sym reserve for rels*)
+val addz_comm = prove_store("addz_comm",
+e0
+(rpt strip_tac >> irule iZ_eq_eq >> rpt strip_tac >>
+ qspecl_then [‘z1’,‘z2’] strip_assume_tac addz_prop6 >>
+ qspecl_then [‘z2’,‘z1’] strip_assume_tac addz_prop7 >>
+ (*once have cond rw test it here*)
+ first_x_assum (qspecl_then [‘u’,‘v’,‘x’,‘y’] assume_tac) >>
+ rfs[] >> rw[rsi_eq_ZR] >> irule eq_ZR >> cheat
+ (*apply Add_sym on one side *))
+(form_goal “!z1 z2. Addz(z1,z2) = Addz(z2,z1)”));
+
+ 
+A r:A ~eq~>A 
+Q >---i---> P(A)
+Thm_2_4
+
+A * -----f------> B
+|               |
+P(A) * ~~~im(f)~~> P(B)
+|                |
+/\               /\
+Q1 ------------> Q2
+
+:Po
+
+
+L (l1 ~ l2) <=> same member 
+
+map: A-> B |-> List(A) -> List(B)
+
+{(0,a),(1,a')} rep of [a,a']
+
+{} 
+
+
+{(0,a),.....,(n,a),.....}
+
+CONS h s = (0,h) INSERT (IMAGE (\(n,e). (n^+,e)) s)
+
+colist: num -> a opt
+
+{} colist empty
+BIGUNION {x | x ⊆ f x}
+
+iscolist(s) <=> 
+?X. ... & IN(s,X)
+
+!e:set of pairs. e in X ==> e = [] | ?h e0. e = e0 :: h0 &
+                            e0 in X
